certicoq/theories/L6_PCPS/shrink_cps_corresp.v
@@ -12,10 +12,14 @@ Require Import Coq.Arith.Arith Coq.NArith.BinNat ExtLib.Data.String ExtLib.Data.
 Require Import Libraries.CpdtTactics Coq.Sorting.Permutation.
 Require Import Libraries.HashMap.
 Require Import Libraries.maps_util.
-
+Require Import Libraries.Coqlib L6.Ensembles_util. 
 Require Import L6.cps.
 Require Import L6.ctx L6.logical_relations.
-Require Import L6.cps_util L6.List_util L6.shrink_cps L6.eval L6.set_util L6.identifiers.
+Require Import L6.cps_util L6.List_util L6.shrink_cps L6.eval L6.set_util L6.identifiers  L6.set_util.
+Require Import L6.shrink_cps_correct.
+
+Locate destructAll.
+
 
 
    Ltac pi0 :=
@@ -28,7 +32,7 @@ Require Import L6.cps_util L6.List_util L6.shrink_cps L6.eval L6.set_util L6.ide
 Notation "A =mgd0= B" := (map_getd_r _ 0 A B) (at level 80).
 Notation "A =mg= B" := (map_get_r _ A B) (at level 81).
 
-
+    
 
 
 Theorem find_def_rename: forall f t xs e sigma fds,
@@ -55,65 +59,6 @@ Proof.
   erewrite IHfds; eauto.
   reflexivity.
 Qed.
-
-
-  (* rewrite rules that 
-    (1) produces a smaller exp
-    (2) preserves the unique binding invariant 
-
-  Fun_split separates a group of mutually recursive functions lrf into two (lf and rf) where the functions bound in rf do not appear in lf 
-     Fun_inline replaces one occurence on f by its definition
-     Fun_dead removes the definition of a set of functions if none of them occur in the rest of the program
-     Constr_dead removes the binding of a datatype when it doesn't appear in the rest of the program 
-     Constr_proj replaces a binding by the nth projection of a datatype when the datatype is known (in ctx) 
-     Constr_case reduces a pattern match into an application of the right continuation on the datatype when the datatype is know (in ctx)
-*)
-  Inductive rw: relation exp :=
-  (* Rules about dead function elimination *)
-| Constr_dead: forall x t ys e, 
-                 num_occur e x 0 ->
-                 rw (Econstr x t ys e) e
-| Prim_dead: forall x p ys e,
-               num_occur e x 0 ->
-               rw (Eprim x p ys e) e
-| Proj_dead: forall x t n y e,
-               num_occur e x 0 ->
-               rw (Eproj x t n y e) e
-| Fun_dead: forall e fds,
-              Forall (fun v => num_occur e v 0) (all_fun_name fds) ->
-              rw (Efun fds e) e 
-| Fun_split: forall lf rf lrf e,
-               split_fds lf rf lrf ->    
-               Forall (fun v => num_occur_fds rf v 0) (all_fun_name lf) ->
-               rw (Efun lrf e) (Efun lf (Efun rf e))
-
-(* Rules about inlining/constant-folding *)
-| Constr_case: forall x c' c'e cl co e c'e' ys,
-      app_ctx c' (Ecase x cl) c'e ->
-      findtag cl co = Some e ->
-      ~bound_var_ctx c' x ->
-      app_ctx c' e c'e' ->      
-      rw (Econstr x co ys c'e) (Econstr x co ys c'e') 
-| Constr_proj: forall v  t t' n x e k ys c' c'e c'e', 
-
-                 app_ctx c' (Eproj v t' n x e) c'e ->
-                 (* nothing shadows constructor x in c' *)
-                 ~ bound_var_ctx c' x ->
-                 (* nothing rebinds the projection k in the rest of the term c' *) 
-                 ~ bound_var e k ->                
-                 nthN ys n = Some k -> 
-                 app_ctx c' (rename k v e) c'e' -> 
-                 rw (Econstr x t ys c'e) (Econstr x t ys c'e')
-| Fun_inline: forall c'  vs c'e f  t xs fb c'e' fds,
-                app_ctx c' (Eapp f t vs) c'e ->
-                ~ bound_var_ctx c' f -> 
-                (*  nothing rebinds vs's in c'e *)
-                Forall (fun v => ~bound_var c'e v) vs -> 
-                get_fun f fds = Some (t, xs, fb) ->
-                app_ctx c' (rename_all (set_list (combine xs vs) (M.empty var)) fb) c'e' ->
-                rw (Efun fds c'e) (Efun fds c'e').                     
-
-
 
 
   Section CENSUS.
@@ -925,3 +870,4800 @@ Qed.
 
 
   End CENSUS.
+
+
+
+
+  
+  Fixpoint inlined_fundefs_f (fds:fundefs) (i:b_map): fundefs :=
+    match fds with
+      | Fnil => Fnil
+      | Fcons f t ys e fds' =>
+        match get_b f i with
+          | true => inlined_fundefs_f fds' i
+          | false => Fcons f t ys e (inlined_fundefs_f fds' i)
+        end
+    end.
+        
+  Theorem inlined_fundefs_append: forall B2 im B1,
+                                    inlined_fundefs_f (fundefs_append B1 B2) im =
+                                    fundefs_append (inlined_fundefs_f B1 im) (inlined_fundefs_f B2 im). 
+  Proof.
+    induction B1; intros; simpl; auto.
+    destruct (get_b v im); auto.
+    rewrite IHB1.
+    simpl. reflexivity.
+  Qed.
+    
+  (* do not inline the first level of functions when going through a Efun2_c?*) 
+  Fixpoint inlined_ctx_f (c:exp_ctx) (i:b_map): exp_ctx :=
+    match c with 
+    | Hole_c => Hole_c
+    | Econstr_c x t ys c => Econstr_c x t ys (inlined_ctx_f c i)
+    | Eproj_c x t n y c => Eproj_c x t n y (inlined_ctx_f c i)
+    | Ecase_c x te t c te' =>
+      Ecase_c x te t (inlined_ctx_f c i) te'
+    | Eprim_c x f ys c => Eprim_c x f ys (inlined_ctx_f c i) 
+    | Efun1_c fds c => Efun1_c (inlined_fundefs_f fds i) (inlined_ctx_f c i) 
+    | Efun2_c cfds e' => Efun2_c (inlined_fundefs_ctx_f cfds i) e'
+    end
+  with inlined_fundefs_ctx_f (cfds: fundefs_ctx) (im:b_map): fundefs_ctx :=
+         match cfds with
+           | Fcons1_c f t ys c fds =>
+             Fcons1_c f t ys (inlined_ctx_f c im) fds
+           | Fcons2_c f t ys e' cfds =>
+             Fcons2_c f t ys e' (inlined_fundefs_ctx_f cfds im)
+         end
+  .
+
+
+  (* collect the names of functions in a term e  which could be affected by inlined_ctx *)
+Inductive fun_names : exp -> Ensemble var :=
+| Fun_Econstr :
+    forall y x t ys e,
+      fun_names e y ->
+      fun_names (Econstr x t ys e) y
+| Fun_Eproj :
+    forall y x tau n y' e,
+      fun_names e y ->
+      fun_names (Eproj x tau n y' e) y
+| Fun_Ecase :
+    forall x y c e B,
+      fun_names e y ->
+      List.In (c, e) B ->
+      fun_names (Ecase x B) y
+| Fun_Efun1 :
+    forall y defs e,
+      fun_names_fundefs defs y ->
+      fun_names (Efun defs e) y
+| Fun_Efun2 :
+    forall y defs e,
+      fun_names e y ->
+      fun_names (Efun defs e) y
+| Fun_Eprim :
+    forall y x p ys e,
+      fun_names e y ->
+      fun_names (Eprim x p ys e) y
+with fun_names_fundefs : fundefs -> Ensemble var :=
+| Fun_Fcons1 :
+    forall f tau ys e defs,
+      fun_names_fundefs (Fcons f tau ys e defs) f
+| Fun_Fcons2 :
+    forall x f tau ys e defs,
+      fun_names_fundefs defs x ->
+      fun_names_fundefs (Fcons f tau ys e defs) x
+| Fun_Fcons3 :
+    forall x f tau ys e defs,
+      fun_names e x ->
+      fun_names_fundefs (Fcons f tau ys e defs) x.
+
+
+Inductive fun_names_ctx: exp_ctx -> Ensemble var  :=
+| Fun_Constr_c: forall c v v' t ys,
+    fun_names_ctx c v ->
+    fun_names_ctx (Econstr_c v' t ys c) v
+| Fun_Proj_c: forall  t n r c v' v,
+                   fun_names_ctx c v' ->
+                   fun_names_ctx (Eproj_c v t n r c) v'
+| Fun_Prim_c: forall  t r c v' v,
+                   fun_names_ctx c v' ->
+                   fun_names_ctx (Eprim_c v t r c) v'
+| Fun_Case1_c: forall v v' lce t c lce',
+     fun_names_ctx c v' ->
+     fun_names_ctx (Ecase_c v lce t c lce') v'
+| Fun_Case2_c: forall v v' e lce t' t c lce',
+                   fun_names e v' ->
+                   List.In (t',e) lce ->
+                   fun_names_ctx (Ecase_c v lce t c lce') v'
+| Fun_Case3_c: forall v v' e lce t' t c lce',
+                   fun_names e v' ->
+                   List.In (t',e) lce' ->
+                   fun_names_ctx (Ecase_c v lce t c lce') v'
+| Fun_Fun11_c: forall fds v c,
+     fun_names_fundefs fds v ->
+     fun_names_ctx (Efun1_c fds c) v
+| Fun_Fun12_c: forall fds v c,
+                  fun_names_ctx c v ->
+                  fun_names_ctx (Efun1_c fds c) v
+| Fun_Fun21_c: forall cfds v e,
+                   fun_names_fundefs_ctx cfds v ->
+                   fun_names_ctx (Efun2_c cfds e) v
+| Fun_Fun22_c: forall cfds v e,
+                   fun_names e v ->
+                   fun_names_ctx (Efun2_c cfds e) v
+with fun_names_fundefs_ctx: fundefs_ctx -> Ensemble var :=
+     | Fun_Fcons11_c: forall f t xs c fds, 
+                          fun_names_fundefs_ctx (Fcons1_c f t xs c fds) f
+     | Fun_Fcons13_c: forall f t xs c fds v,
+                          fun_names_ctx c v ->
+                           fun_names_fundefs_ctx (Fcons1_c f t xs c fds) v
+     | Fun_Fcons14_c: forall f t xs c fds v,
+                          fun_names_fundefs fds v ->
+                          fun_names_fundefs_ctx (Fcons1_c f t xs c fds) v
+
+     | Fun_Fcons21_c: forall f t xs e cfds, 
+                          fun_names_fundefs_ctx (Fcons2_c f t xs e cfds) f
+     | Fun_Fcons23_c: forall f t xs e cfds v,
+                          fun_names e v ->
+                          fun_names_fundefs_ctx (Fcons2_c f t xs e cfds) v
+     | Fun_Fcons24_c: forall f t xs e cfds v,
+                          fun_names_fundefs_ctx cfds v ->
+                          fun_names_fundefs_ctx (Fcons2_c f t xs e cfds) v.
+
+  
+
+ Definition eq_b_map_P:  Ensemble var -> b_map -> b_map -> Prop :=
+    fun S rho1 rho2 =>
+      forall x, S x -> get_b x rho1 = get_b x rho2.
+
+
+ Theorem eq_b_map_P_mon:
+   forall S S' b1 b2,
+   eq_b_map_P S' b1 b2 ->
+   Included _ S S' ->
+   eq_b_map_P S b1 b2.
+ Proof.
+   intros.
+   intro; intros.
+   apply H0 in H1. apply H in H1. auto.
+ Qed.
+   
+  Theorem  eq_b_inlined_fundefs: forall b1 b2 fds,
+      eq_b_map_P (name_in_fundefs fds) b1 b2 -> 
+inlined_fundefs_f fds b1 = inlined_fundefs_f fds b2.
+  Proof.
+    induction fds; intros.
+    - simpl in *.
+      assert ( eq_b_map_P (name_in_fundefs fds) b1 b2 ).
+      eapply eq_b_map_P_mon; eauto with Ensembles_DB.
+      specialize (IHfds H0).      
+      destruct (get_b v b1) eqn:gbv1.
+      rewrite H in gbv1.
+      rewrite gbv1.
+      apply IHfds.
+      left; auto.
+      rewrite H in gbv1.
+      rewrite gbv1.
+      rewrite IHfds.
+      auto.
+      left; auto.
+    - auto.
+  Qed.
+  
+(*  Theorem eq_b_map_inlined_ctx_mut:
+   forall b1 b2,
+   (forall c,
+     eq_b_map_P (fun_names_ctx c) b1 b2 ->
+      inlined_ctx_f c b1 = inlined_ctx_f c b2) /\
+     (forall fds,
+     eq_b_map_P (fun_names_fundefs_ctx fds) b1 b2 ->
+      inlined_fundefs_ctx_f fds b1 = inlined_fundefs_ctx_f fds b2).
+ Proof.
+   Admitted.*)
+
+
+  Print Dom_map.
+  Definition Dom_map_b im: Ensemble var :=
+    fun x => get_b x im = true.
+  
+  Theorem inlined_comp_ctx: (forall c1 c2 im,  
+                              inlined_ctx_f (comp_ctx_f c1 c2) im = comp_ctx_f (inlined_ctx_f c1 im) (inlined_ctx_f c2 im))
+                            /\
+                             (forall f c2 im, (inlined_fundefs_ctx_f (comp_f_ctx_f f c2) im)  =
+                                             (comp_f_ctx_f (inlined_fundefs_ctx_f f im) (inlined_ctx_f c2 im)))
+  .
+  Proof.
+    exp_fundefs_ctx_induction IHc1 IHf; intros; simpl; auto; try (    rewrite IHc1; reflexivity).
+    rewrite IHf. reflexivity.
+    rewrite IHf. reflexivity.
+  Qed.
+  
+  Theorem Disjoint_inlined_fds:
+    forall fds im,
+      Disjoint _ (bound_var_fundefs fds) (Dom_map_b im) ->
+      inlined_fundefs_f fds im = fds.
+  Proof.
+    induction fds; intros.
+    - rewrite bound_var_fundefs_Fcons in H.
+      simpl.
+      destruct (get_b v im) eqn:bvm.
+      + exfalso.
+        inv H. specialize (H0 v).
+        apply H0; split; auto.
+      + rewrite IHfds.
+        reflexivity.
+        eapply Disjoint_Included_l.
+        2: apply H.
+        eauto with Ensembles_DB.
+    - reflexivity.
+Qed.     
+    
+  Theorem Disjoint_inlined_ctx_mut:
+    forall im,
+    (forall c,
+      Disjoint _ (bound_var_ctx c) (Dom_map_b im) ->
+      inlined_ctx_f c im = c) /\
+    (forall fc,
+       Disjoint _ (bound_var_fundefs_ctx fc) (Dom_map_b im) ->
+     inlined_fundefs_ctx_f fc im = fc).
+  Proof.
+    intro im.
+    exp_fundefs_ctx_induction IHc IHf; simpl; intros; try (rewrite IHc); try (rewrite IHf); auto.
+    - eapply Disjoint_Included_l.
+      2: apply H.
+      rewrite bound_var_Econstr_c.
+      left; auto.
+    - eapply Disjoint_Included_l.
+      2: apply H.
+      rewrite bound_var_Eproj_c.
+      left; auto.
+    - eapply Disjoint_Included_l.
+      2: apply H.
+      rewrite bound_var_Eprim_c.
+      left; auto.
+    - eapply Disjoint_Included_l.
+      2: apply H.
+      intro; intro.
+      apply Bound_Case1_c. auto.
+    - rewrite Disjoint_inlined_fds.
+      reflexivity.
+      eapply Disjoint_Included_l.
+      2: apply H.      
+      rewrite bound_var_Fun1_c.
+      left; auto.
+    - eapply Disjoint_Included_l.
+      2: apply H.      
+      rewrite bound_var_Fun1_c.
+      right; auto.
+    - eapply Disjoint_Included_l.
+      2: apply H.
+      rewrite bound_var_Fun2_c.
+      left; auto.
+    - eapply Disjoint_Included_l.
+      2: apply H.
+      rewrite bound_var_Fcons1_c.
+      right; right; left; auto.
+    - eapply Disjoint_Included_l.
+      2: apply H.
+      rewrite bound_var_Fcons2_c.
+      right; right; right; auto.
+  Qed.
+
+
+  Theorem Disjoint_inlined_ctx:
+    (forall c im,
+      Disjoint _ (bound_var_ctx c) (Dom_map_b im) ->
+      inlined_ctx_f c im = c).
+  Proof.
+    intros.
+    apply Disjoint_inlined_ctx_mut.
+    auto.
+  Qed.
+
+    
+  Section CONTRACT.
+
+    (* may need to also have count = 0 *)
+    Definition inl_inv (im:b_map) (sub:ctx_map) (e:exp):Prop :=
+      forall f, get_b f im = true ->
+                ~ (bound_var e f) /\
+                (forall t xs m, M.get f sub = Some (SVfun t xs m) ->
+                             Disjoint _ (bound_var e) (FromList xs)).
+
+    
+    Definition cmap_view_ctx sub c: Prop :=
+      (forall x t xs,
+         M.get x sub = Some (SVconstr t xs) <->
+         exists c' c'',
+           c = comp_ctx_f c' (Econstr_c x t xs c'')) /\
+      (forall f t ys e,
+         M.get f sub = Some (SVfun t ys e) <->
+       exists c' c'' B1 B2,
+         c = comp_ctx_f c' (Efun1_c
+                           (fundefs_append B1 (Fcons f t ys e B2)) c'')).
+
+    Theorem empty_view_hole:
+      cmap_view_ctx (M.empty _) (Hole_c).
+    Proof.
+      split; split; intros.
+      - rewrite M.gempty in H. inv H.
+      - destructAll.
+        exfalso.
+        destruct x0; inv H.
+      - rewrite M.gempty in H. inv H.
+      - destructAll.
+        exfalso.
+        destruct x; inv H.
+    Qed.
+        
+    (* This is implied by sig_inv_dom in the case where e is also closed.
+   Note 12/16/16: if sig_inv_dom has both ~ bv and ~ fv, then we should be able to prove corresp of contract for ub w/o closed top level 
+  *) 
+    Definition sig_inv sig e: Prop := 
+      forall x y, M.get x sig = Some y ->
+                  (* dom *) ~ (bound_var e x) /\
+                            (* codom *)
+                            (num_occur e y  0 \/ bound_var e y).
+
+
+    
+    (* meaning either get_c y count 0 OR y is bound on the way to the hole [or, weaker, bound somewhere in the term, which is enough to show that Disjoint Dom Codom *)
+    Theorem not_free_bound_or_not_occur :
+      forall v : var,
+        (forall e : exp,  ~ occurs_free e v -> num_occur e v 0  \/ bound_var e v) /\
+        (forall f : fundefs, ~ occurs_free_fundefs f v ->  num_occur_fds f v 0 \/ bound_var_fundefs f v).
+    Proof.
+      intro v.
+      apply exp_def_mutual_ind; intros.
+      - destruct (var_dec v0 v).
+        + right. subst.
+          constructor.
+        + assert (~ List.In v l).
+          intro; apply H0.
+          constructor; auto.
+          assert (~ (occurs_free e) v).
+          intro; apply H0.
+          constructor 2; auto.
+          apply H in H2. inv H2.
+          left.
+          apply not_occur_list_not_in in H1.
+          eapply num_occur_n. constructor.
+          apply H3.
+          rewrite H1. auto.
+          right.
+          apply bound_var_Econstr.
+          left; auto.
+      - left.
+        eapply num_occur_n.
+        constructor.
+        constructor.
+        simpl.
+        destruct (cps_util.var_dec v v0).
+        exfalso; apply H.
+        subst. constructor.
+        auto.
+      - assert (~occurs_free e v).
+        intro; apply H1.
+        constructor. auto.
+        assert (~ occurs_free (Ecase v0 l) v).
+        intro; apply H1.
+        apply Free_Ecase3. auto.
+        apply H in H2.
+        apply H0 in H3.
+        inv H2.
+        inv H3.
+        left.
+        inv H2. rewrite H8.
+        eapply num_occur_n.
+        constructor. constructor.
+        apply H4. apply H7.
+        simpl. destruct (cps_util.var_dec v v0).
+        inv H8.
+        auto.
+        right.
+        apply bound_var_Ecase_cons. right; auto.
+        right. apply bound_var_Ecase_cons. auto.
+      - destruct (var_dec v0 v).
+        right; subst; constructor.
+        assert (~ occurs_free e v).
+        intro; apply H0.
+        constructor. auto. auto.
+        apply H in H1.
+        destruct H1. left.
+        eapply num_occur_n.
+        constructor; eauto.
+        simpl.
+        destruct (cps_util.var_dec v v1).
+        exfalso; apply H0; subst; constructor.
+        auto.
+        right; auto.
+      - assert ( ~ occurs_free_fundefs f2 v).
+        intro.
+        apply H1.        
+        apply Free_Efun2. auto.
+        assert (Hf2 := Decidable_name_in_fundefs f2).
+        destruct Hf2.
+        specialize (Dec v).
+        destruct Dec.
+        + right. constructor. apply name_in_fundefs_bound_var_fundefs. auto.
+        + assert (~ occurs_free e v).
+          intro.
+          apply H1.
+          constructor; auto.
+          apply H0 in H4.
+          apply H in H2.
+          inv H4.
+          inv H2.
+          left.
+          eapply num_occur_n. constructor; eauto. auto.
+          right; auto.
+          right; auto.
+      - left.
+        eapply num_occur_n. constructor.
+        simpl.
+        destruct (cps_util.var_dec v v0).
+        exfalso; apply H; subst; auto.
+        apply not_occur_list_not_in.
+        intro; apply H.
+        constructor.
+        auto.
+      - destruct (var_dec v0 v).
+        + right. subst.
+          constructor.
+        + assert (~ List.In v l).
+          intro; apply H0.
+          constructor; auto.
+          assert (~ (occurs_free e) v).
+          intro; apply H0.
+          apply Free_Eprim2; auto.
+          apply H in H2.  inv H2.
+          left.
+          apply not_occur_list_not_in in H1.
+          eapply num_occur_n. constructor.
+          apply H3.
+          rewrite H1. auto.
+          right.
+          apply bound_var_Eprim.
+          left; auto.
+      - left.
+        eapply num_occur_n.
+        constructor.
+        simpl.
+        destruct (cps_util.var_dec v v0).
+        exfalso; apply H; subst; auto.
+        auto.
+      - destruct (var_dec v0 v).
+        right; subst; auto.
+        assert (Hl := Decidable_FromList l).
+        inv Hl. specialize (Dec v). inv Dec.
+        right.
+        constructor. right; auto.
+        assert (Hf5 := Decidable_name_in_fundefs f5).
+        destruct Hf5; specialize (Dec v); inv Dec.
+        right. constructor 2. apply name_in_fundefs_bound_var_fundefs. auto.
+        assert (~ occurs_free e v).
+        intro; apply H1.
+        constructor; auto.
+        apply H in H4.
+        assert (~ occurs_free_fundefs f5 v).
+        intro; apply H1.
+        constructor 2; auto.
+        apply H0 in H5.
+        destruct H4.
+        destruct H5.
+        left.
+        eapply num_occur_fds_n.
+        constructor; eauto. auto.
+        right.
+        constructor 2. auto.
+        right. auto.
+      - left; constructor.
+    Qed.
+
+
+
+      
+      
+          
+        
+    Theorem Disjoint_apply_r: forall sig x,
+      Disjoint _ (Dom_map sig) (Singleton _ x) ->
+      apply_r sig x = x.
+    Proof.
+      intros.
+      unfold apply_r.
+      destruct (M.get x sig) eqn:gxs.
+      exfalso; inv H. specialize (H0 x).
+      apply H0.
+      split; auto. exists e. auto.
+      auto.
+    Qed.      
+      
+    Theorem Disjoint_apply_r_FromList: forall sig l,
+      Disjoint _ (Dom_map sig) (FromList l) ->
+      apply_r_list sig l = l. 
+    Proof.
+      induction l; intros.
+      - auto.
+      - simpl. rewrite IHl.
+        rewrite Disjoint_apply_r.
+        auto.
+        eapply Disjoint_Included_r.
+        2: apply H. rewrite FromList_cons; auto with Ensembles_DB.
+        eapply Disjoint_Included_r.
+        2: apply H. rewrite FromList_cons; auto with Ensembles_DB.
+    Qed.        
+
+    Theorem Disjoint_Setminus_swap:
+      forall {A} s1 s2 s3,
+        Disjoint A (Setminus _ s1 s2) s3 <-> Disjoint A s1 (Setminus _ s3 s2).
+    Proof.
+      intros. split; intro.
+      - split; intro; intro.
+        inv H. specialize (H1 x).
+        apply H1.
+        inv H0.
+        inv H2.
+        split;
+        eauto with Ensembles_DB.
+        split; auto.
+      - split; intro; intro.
+        inv H.
+        inv H0.
+        specialize (H1 x).
+        inv H.
+        apply H1. split.
+        auto.
+        split; auto.
+    Qed.
+
+    Theorem same_name_in_fun: forall f,
+      Same_set _ (name_in_fundefs f) (FromList (all_fun_name f)).
+    Proof.
+      intro.
+      split; intro; intro; apply name_fds_same; auto.
+    Qed.
+      
+      
+    Theorem Disjoint_Dom_map_funs: forall f2 sig s,
+      
+      Disjoint _ (Dom_map sig) (Setminus _ s (name_in_fundefs f2)) -> 
+      
+      Disjoint M.elt (Dom_map (remove_all sig (all_fun_name f2))) s.
+    Proof.
+      intros.
+      rewrite Dom_map_remove_all.
+      apply Disjoint_Setminus_swap.
+      rewrite same_name_in_fun in H.
+      auto.
+    Qed.
+
+        
+    
+    Theorem Disjoint_dom_rename_all:
+      (forall  e sig,
+         Disjoint _ (Dom_map sig) (occurs_free e) ->
+         rename_all sig e = e) /\
+      (forall f sig,
+         Disjoint _ (Dom_map sig) (Union _ (occurs_free_fundefs f) (name_in_fundefs f)) ->
+        rename_all_fun sig f = f).
+    Proof.
+      apply exp_def_mutual_ind; intros; repeat normalize_occurs_free_in_ctx; simpl.
+      - rewrite H.
+        rewrite Disjoint_apply_r_FromList.
+        reflexivity.        
+        eapply Disjoint_Included_r.
+        2: apply H0. auto with Ensembles_DB.
+        rewrite Dom_map_remove.
+        split.
+        intros. intro.
+        inv H1.
+        destruct (var_dec v x). subst.
+        inv H2. apply H4. auto.
+        inv H0. specialize (H1 x).
+        apply H1. split.
+        apply H2.
+        right.
+        split; auto.
+        intro; apply n.
+        inv H0. auto.
+      - rewrite Disjoint_apply_r; auto.
+      - assert ( Disjoint M.elt (Dom_map sig) (occurs_free (Ecase v l)) ).
+        eauto with Ensembles_DB.
+        apply H0 in H2.
+        simpl in H2.
+        inversion H2.
+        rewrite  H4.
+        rewrite H4.
+        rewrite H5.
+        rewrite H5.
+        rewrite H; auto with Ensembles_DB.        
+      - rewrite Disjoint_apply_r.
+        rewrite H; auto.
+        rewrite Dom_map_remove.
+        rewrite Disjoint_Setminus_swap.
+        eapply Disjoint_Included_r.
+        2: apply H0.
+        right; auto.
+        eapply Disjoint_Included_r.
+        2: apply H0.
+        left; auto.
+      -  rewrite H.
+         rewrite H0.
+         auto.         
+         apply Disjoint_Dom_map_funs.
+         auto with Ensembles_DB.
+         apply Disjoint_Dom_map_funs.
+         eapply Disjoint_Included_r.
+         2: apply H1. eauto with Ensembles_DB.
+      - rewrite Disjoint_apply_r.
+        rewrite Disjoint_apply_r_FromList.
+        auto.
+        eauto with Ensembles_DB.
+        eauto with Ensembles_DB.
+      - rewrite Disjoint_apply_r_FromList.
+        rewrite H.
+        auto.
+        rewrite Dom_map_remove.
+        rewrite Disjoint_Setminus_swap.
+        auto with Ensembles_DB.
+        auto with Ensembles_DB.
+      - rewrite Disjoint_apply_r.
+        auto.
+        rewrite occurs_free_Ehalt in H.
+        auto.
+      -  rewrite H.
+         rewrite H0.
+         auto.
+         { simpl in H1.
+           split; intro; intro.
+           inv H2.
+           inv H1.
+           specialize (H2 x).
+           apply H2.
+           destruct (var_dec x v).
+           subst; auto.           
+           inv H4.
+           split. auto.
+           left.
+           right. split; auto. intro; apply n.
+           inv H4; auto.
+           split; auto.
+         }         
+         simpl in H1.
+         rewrite Dom_map_remove_all.
+         rewrite Disjoint_Setminus_swap.
+         eapply Disjoint_Included_r.
+         2: apply H1.
+         intro.
+         intro.
+         assert (Hd := Decidable_name_in_fundefs f5).
+         inv Hd.
+         specialize (Dec x).
+         inv Dec; 
+           auto with Ensembles_DB.
+         destruct (var_dec x v).
+         right. subst; left; auto.
+         left.
+         inv H2.
+         left.       
+         split; auto.         
+         intro.
+         inv H2; auto.
+         inv H6; auto.
+         inv H6; auto.
+      -                 reflexivity.
+    Qed.
+
+    
+
+    
+    
+(* split sig_inv into the comps *)
+    Definition sig_inv_dom (sig:r_map) e: Prop := 
+      forall x y, M.get x sig = Some y ->
+                  ~ (bound_var e x).
+
+
+
+    
+    Definition sig_inv_dom_fundefs (sig:r_map) fds: Prop := 
+      forall x y, M.get x sig = Some y ->
+                  ~ (bound_var_fundefs fds x).
+
+
+    Definition sig_inv_dead (sig:r_map) e :Prop :=
+      forall x y, M.get x sig = Some y ->
+                 num_occur e x 0.
+
+    Definition sig_inv_dead_fundefs (sig:r_map) f :Prop :=
+      forall x y, M.get x sig = Some y ->
+                  num_occur_fds f x 0.
+
+    
+    Definition sig_inv_codom (sig:r_map) e: Prop := 
+      forall x y, M.get x sig = Some y ->
+                   ~ (occurs_free e y).
+
+
+    Theorem sig_inv_implies_dom:
+      forall sig e,
+        sig_inv sig e ->
+        sig_inv_dom sig e.
+    Proof.
+      intros. intro. intros.
+      apply H in H0. destructAll; auto.
+    Qed.
+
+
+
+        
+      
+
+    Theorem inl_inv_mon:
+      forall e' e im sub ,
+      Included _ (bound_var e') (bound_var e) ->
+      inl_inv im sub e ->
+      inl_inv im sub e'.
+    Proof.
+      intros; intro; intros.
+      apply H0 in H1; destructAll.
+      split; intro; intros.
+      - apply H1. apply H; auto.
+      - apply H2 in H3.
+        eapply Disjoint_Included_l.
+        2: apply H3. auto.
+    Qed.
+
+        
+    Theorem sig_inv_dom_mon:
+      forall e' e sig,
+      Included _ (bound_var e') (bound_var e) ->
+      sig_inv_dom sig e ->
+      sig_inv_dom sig e'.
+    Proof.
+      intros. intro; intros.
+      apply H0 in H1.
+      intro.
+      apply H1.
+      apply H. auto.
+    Qed.
+
+    Theorem sig_inv_dom_fundefs_antimon:
+      forall fds' fds sig,
+        Included _ (bound_var_fundefs fds') (bound_var_fundefs fds) ->
+        sig_inv_dom_fundefs sig fds ->
+        sig_inv_dom_fundefs sig fds'.
+    Proof.
+      intros. 
+      intro; intros.
+      apply H0 in H1.
+      intro; apply H1.
+      apply H; auto.
+    Qed.
+      
+    Theorem bound_var_subterm_e:
+      forall e e', 
+      subterm_e e e' ->
+      Included _ (bound_var e) (bound_var e').
+    Proof.
+      intros.
+      induction H.
+      inv H; repeat normalize_bound_var; eauto with Ensembles_DB.
+      intro. intro.
+      eapply Bound_Ecase; eauto.
+      left.
+      revert H H0.
+      revert x0.
+      induction fds; intros.
+      rewrite bound_var_fundefs_Fcons.
+      inv H0; auto.
+      inv H0.            
+      eapply Included_trans; eauto.
+    Qed.
+
+
+    Theorem dsubterm_num_occur:
+      (forall {e' e} {x} {n m},
+         dsubterm_e e e' ->
+      num_occur e' x n ->
+      num_occur e x m ->
+      m <= n) /\
+      (forall {f} {e} {x} {n m},
+         dsubterm_fds_e e f ->
+         num_occur_fds f x n ->
+         num_occur e x m ->
+         m <= n).
+    Proof.      
+     eapply exp_def_mutual_ind; intros.
+     - inv H0; inv H1.
+       assert (m = n0).
+       eapply (proj1 (num_occur_det _)); eauto.
+       omega.
+     - inv H.
+       inv H4.
+     - inv H2.
+       inv H8.
+       inv H1.
+       inv H5.
+       + inv H1.
+         assert (m = n).
+         eapply (proj1 (num_occur_det _)); eauto.
+         omega.
+       + assert (m <=  num_occur_list [v] x + m0).
+         eapply H0.
+         eapply dsubterm_case.
+         apply H1.
+         constructor; auto.
+         auto.
+         omega.
+     - inv H0; inv H1.
+       assert (m = n1).
+       eapply (proj1 (num_occur_det _)); eauto.
+       omega.
+     - inv H2.
+       inv H1.
+       specialize (H _ _ _ _ H5 H9 H3).
+       omega.
+       assert (n0 = m).
+       eapply (proj1 (num_occur_det _)); eauto.
+       omega.       
+     - inv H.
+     - inv H0; inv H1.
+       assert (m = n0).
+       eapply (proj1 (num_occur_det _)); eauto.
+       omega.
+     - inv H.
+     - inv H2.
+       inv H1.
+       + assert (m = n0).
+       eapply (proj1 (num_occur_det _)); eauto.
+       omega.
+       + specialize (H0 _ _ _ _ H5 H12 H3).
+         omega.
+     - inv H.
+    Qed.
+
+    Theorem subterm_num_occur:
+      forall {e e'} {x} ,
+        subterm_e e e' ->
+        forall {n m},
+        num_occur e x m ->
+        num_occur e' x n ->
+        m <= n.
+    Proof.
+      intros e e' x H.
+      induction H.
+      - intros.
+        eapply (proj1 dsubterm_num_occur); eauto.
+      - intros.
+        assert (exists z, num_occur y x z).
+        eapply e_num_occur. inv H3.
+        specialize (IHclos_trans1 _ _ H1 H4).
+        specialize (IHclos_trans2 _ _ H4 H2).
+        omega.
+    Qed.
+
+
+    Theorem subterm_sig_dead:
+      forall {e e'},
+        subterm_e e e' ->
+        forall {sig}, 
+        sig_inv_dead sig e' ->
+        sig_inv_dead sig e.
+    Proof.
+      intros.
+      intro. intros.
+      apply H0 in H1.
+      assert (exists y, num_occur e x y) by apply e_num_occur.
+      inv H2.
+      assert (x0 <= 0).
+      eapply subterm_num_occur; eauto.
+      apply le_n_0_eq in H2. subst; auto.
+    Qed.
+
+
+    Theorem rename_sig_dead:
+      forall {sig} {e},
+      sig_inv_dead sig e -> 
+      rename_all sig e = e.
+    Proof.
+      intros.
+      apply Disjoint_dom_rename_all.
+      split. intro. intro.
+      inv H0.
+      inv H1. apply H in H0.
+      revert H2.    
+      apply not_occurs_not_free. auto.
+    Qed.
+
+
+    Theorem sig_inv_closed_dead:
+      forall {sig} {e},
+        sig_inv sig e ->
+        closed e ->
+        sig_inv_dead sig e.
+    Proof.
+      intros. intro. intros.
+      apply H in H1.
+      destructAll.
+      assert (~ occurs_free e x).
+      intro.
+      apply H0 in H3. inv H3.
+      apply not_free_bound_or_not_occur in H3.
+      inv H3; auto.
+      exfalso; auto.
+    Qed.
+    
+    Theorem remove_all_list_no_shadow:
+      forall l sig,
+      (forall x, (exists y, M.get x sig = Some y) -> ~ FromList l x) ->
+        remove_all sig l =mg= sig.
+    Proof.
+      induction l; intros.
+      - apply smg_refl.
+      - simpl. eapply smg_trans.
+        2: apply IHl.
+        apply prop_remove_all.
+        apply remove_none.
+        destruct (M.get a sig) eqn:gas.
+        exfalso.
+        specialize (H a).
+        destruct H.
+        eauto.
+        constructor.
+        auto.
+        auto.
+        intros.
+        destruct H0.
+        intro.
+        eapply H.
+        eexists; eauto.
+        constructor 2; auto.
+    Qed.        
+        
+    Theorem remove_all_fun_name_no_shadow:
+      forall f2 sig,
+      sig_inv_dom_fundefs sig f2 -> 
+      remove_all sig (all_fun_name f2) =mg= sig.
+    Proof.
+      induction f2.
+      - intros. simpl.
+        assert (sig_inv_dom_fundefs sig f2).
+        eapply sig_inv_dom_fundefs_antimon; eauto.
+        normalize_bound_var. right; auto.
+        apply IHf2 in H0.
+        eapply smg_trans.
+        2: apply H0.        
+        apply prop_remove_all.
+        apply remove_none.
+        destruct (M.get v sig) eqn:gvs.
+        exfalso.
+        apply H in gvs.
+        apply gvs.
+        apply bound_var_fundefs_Fcons.
+        auto.
+        auto.
+      - intros. apply smg_refl.
+    Qed.
+    
+    Theorem rename_all_no_shadow:
+      forall sig,
+        (forall e,
+        sig_inv_dom sig e ->
+        rename_all sig e = rename_all_ns sig e) /\
+        (forall fds,
+           sig_inv_dom_fundefs sig fds -> 
+           rename_all_fun sig fds = rename_all_fun_ns sig fds)
+         .         
+    Proof.
+      intro sig.
+      apply exp_def_mutual_ind; intros; simpl.
+      - assert (sig_inv_dom sig e).
+        eapply sig_inv_dom_mon.
+        2: apply H0.
+        apply bound_var_subterm_e.
+        constructor; constructor.
+        apply H in H1.
+        erewrite (proj1 prop_rename_all). rewrite H1.
+        reflexivity.
+        apply remove_none.
+        destruct (M.get v sig) eqn:gvs.
+        exfalso.
+        apply H0 in gvs.
+        apply gvs.
+        auto.
+        auto.
+      - reflexivity.
+      - rewrite H.
+        assert ( sig_inv_dom sig (Ecase v l)).
+        intro. intros.
+        intro.
+        apply H1 in H2.
+        apply H2.
+        inv H3.
+        eapply Bound_Ecase; eauto.
+        right. eauto.
+        apply H0 in H2.
+        simpl in H2. inv H2.
+        reflexivity.
+        intro. intros.
+        intro.
+        apply H1 in H2.
+        apply H2.
+        eapply Bound_Ecase.
+        apply H3.
+        constructor. auto.        
+      - assert (sig_inv_dom sig e).
+        eapply sig_inv_dom_mon.
+        2: apply H0.
+        apply bound_var_subterm_e.
+        constructor; constructor.
+        apply H in H1.
+        erewrite (proj1 prop_rename_all). rewrite H1.
+        reflexivity.
+        apply remove_none.
+        destruct (M.get v sig) eqn:gvs.
+        exfalso.
+        apply H0 in gvs.
+        apply gvs.
+        auto.
+        auto.
+      - assert (sig_inv_dom_fundefs sig f2).
+        intro. intros.
+        apply H1 in H2.
+        intro; apply H2.
+        apply bound_var_Efun.
+        auto.        
+        assert  (remove_all sig (all_fun_name f2) =mg= sig).
+        apply remove_all_fun_name_no_shadow.
+        auto.
+        erewrite (proj1 prop_rename_all); eauto.
+        rewrite H0.
+        erewrite (proj2 prop_rename_all); eauto.
+        rewrite H.
+        reflexivity.
+        auto.
+        eapply sig_inv_dom_mon.
+        2: apply H1.
+        rewrite bound_var_Efun. right; auto.
+      - reflexivity.
+      - assert (sig_inv_dom sig e).
+        eapply sig_inv_dom_mon.
+        2: apply H0.
+        apply bound_var_subterm_e.
+        constructor; constructor.
+        apply H in H1.
+        erewrite (proj1 prop_rename_all). rewrite H1.
+        reflexivity.
+        apply remove_none.
+        destruct (M.get v sig) eqn:gvs.
+        exfalso.
+        apply H0 in gvs.
+        apply gvs.
+        auto.
+        auto.
+      - reflexivity.
+      - erewrite (proj1 prop_rename_all).
+        rewrite H.
+        rewrite H0.
+        reflexivity.
+        eapply sig_inv_dom_fundefs_antimon; eauto.
+        rewrite bound_var_fundefs_Fcons.
+        right; auto.
+        intro. intros.
+        apply H1 in H2.
+        intro; apply H2.
+        apply bound_var_fundefs_Fcons.
+        auto.
+        apply remove_all_list_no_shadow.
+        intros.
+        destruct H2.
+        apply H1 in H2.
+        intro; apply H2.
+        apply bound_var_fundefs_Fcons.
+        auto.
+      - reflexivity.
+    Qed.
+
+         Theorem rename_all_ns_empty: (forall e,
+                             e = rename_all_ns (M.empty var) e) /\
+                          (forall fds, fds = rename_all_fun_ns (M.empty var) fds).
+        Proof.
+          split; intros.
+          rewrite <- (proj1 (rename_all_no_shadow _)).
+          apply rename_all_empty.
+          intro. intros. rewrite M.gempty in H. inv H.
+          rewrite <- (proj2 (rename_all_no_shadow _)).
+          apply rename_all_empty.
+          intro. intros. rewrite M.gempty in H. inv H.
+        Qed.
+
+        Theorem rename_all_ns_app_ctx:
+          forall e sig, 
+            (forall c,
+               rename_all_ns sig (c |[ e]|) =
+               (rename_all_ctx_ns sig c) |[rename_all_ns sig e ]|) /\
+            (forall fc,
+               rename_all_fun_ns sig (fc <[ e]>) =
+               (rename_all_fun_ctx_ns sig fc) <[rename_all_ns sig e ]>)
+             .
+             Proof.
+               intros.
+               exp_fundefs_ctx_induction IHc IHfc; simpl; auto; try (rewrite IHc; auto); try (rewrite IHfc; auto).
+               intro. 
+               rewrite list_append_map.
+               simpl.
+               rewrite IHc; auto.
+             Qed.
+
+
+             Theorem rename_all_ctx_ns_comp_ctx:
+               forall c' sig, 
+            (forall c,
+               rename_all_ctx_ns sig (comp_ctx_f c c') =
+               comp_ctx_f (rename_all_ctx_ns sig c) (rename_all_ctx_ns sig c')) /\
+            (forall fc,
+               rename_all_fun_ctx_ns sig (comp_f_ctx_f fc c') =
+               comp_f_ctx_f (rename_all_fun_ctx_ns sig fc) (rename_all_ctx_ns sig c'))
+             .
+ intros.
+               exp_fundefs_ctx_induction IHc IHfc; simpl; auto; try (rewrite IHc; auto); try (rewrite IHfc; auto).
+             Qed.
+             
+               
+             
+             
+             Theorem rename_all_ns_fundefs_append:
+               forall sig B2 B1,
+                 rename_all_fun_ns sig (fundefs_append B1 B2) =
+                 fundefs_append (rename_all_fun_ns sig B1) (rename_all_fun_ns sig B2).
+             Proof.
+               induction B1; simpl; auto.
+               rewrite IHB1. auto.
+             Qed.               
+
+             Theorem bound_var_rename_all_ns:
+               forall sigma, 
+                 (forall (e : exp),
+                    bound_var e <--> bound_var (rename_all_ns sigma e)) /\
+                 (forall (fds : fundefs),
+                    bound_var_fundefs fds <--> bound_var_fundefs (rename_all_fun_ns sigma fds)).
+             Proof.
+               intro sig.
+               apply exp_def_mutual_ind; intros; simpl; repeat (normalize_bound_var); split; try (rewrite H); try (rewrite H0); auto with Ensembles_DB.
+             Qed.
+                 
+    Theorem all_fun_name_append:
+      forall B2 B1,
+      all_fun_name (fundefs_append B1 B2) = all_fun_name B1 ++ all_fun_name B2.
+    Proof.
+      induction B1; auto.
+      simpl.
+      rewrite IHB1. auto.
+    Qed.      
+
+
+    Theorem remove_all_append:
+      forall B2 B1 sig,
+      remove_all sig (B1++B2) = remove_all (remove_all sig B1) B2.
+    Proof.
+      induction B1; auto.
+      intro.
+      simpl.
+      erewrite IHB1. auto.
+    Qed.
+
+       Corollary ub_app_ctx_exp:
+         forall c e v,
+           unique_bindings (c |[ e ]|) ->
+           bound_var e v ->
+           ~ bound_var_ctx c v. 
+       Proof.
+         intros.
+         apply ub_app_ctx_f in H.
+         destructAll.
+         inv H2. specialize (H3 v).
+         intro; apply H3.
+         split; auto.
+       Qed.
+
+       Print name_in_fundefs.
+(* Section move_to_identifiers. *)
+       Fixpoint name_in_ctx_fundefs B:=
+         match B with
+           | Fcons1_c f' _ _ _ B0 => Union var [set f'] (name_in_fundefs B0)
+           | Fcons2_c f' _ _ _ B0 => Union var [set f'] (name_in_ctx_fundefs B0)
+         end.
+
+       Theorem name_in_ctx_fundefs_ctx:
+         forall e cf, 
+           Same_set _ (name_in_ctx_fundefs cf) (name_in_fundefs (cf <[ e ]>)).
+       Proof.
+         induction cf.
+         simpl. eauto with Ensembles_DB.
+         simpl. rewrite IHcf.
+         eauto with Ensembles_DB.
+       Qed.         
+         
+       Inductive occurs_free_ctx : exp_ctx -> Ensemble var :=
+       | Free_Econstr1 :
+           forall y x t ys e,
+             List.In y ys ->
+             occurs_free_ctx (Econstr_c x t ys e) y
+       | Free_Econstr2 :
+           forall y x t ys e,
+             ~ x = y ->
+             occurs_free_ctx e y ->
+             occurs_free_ctx (Econstr_c x t ys e) y
+       | Free_Ecase1 :
+           forall x cl1 c e cl2, 
+             occurs_free_ctx (Ecase_c x cl1 c e cl2) x
+       | Free_Ecase2 :  
+           forall y x cl1 c e cl2,
+             occurs_free_ctx e y ->
+             occurs_free_ctx (Ecase_c x cl1 c e cl2) y
+       | Free_Ecase3 :  
+           forall y x cl1 c e cl2,
+             occurs_free (Ecase x cl1) y ->
+             occurs_free_ctx (Ecase_c x cl1 c e cl2) y
+       | Free_Ecase4 :  
+           forall y x cl1 c e cl2,
+             occurs_free (Ecase x cl2) y ->
+             occurs_free_ctx (Ecase_c x cl1 c e cl2) y
+       | Free_Eproj1 :
+           forall y x tau n e,
+             occurs_free_ctx (Eproj_c x tau n y e) y
+       | Free_Eproj2 :
+           forall y x tau n y' e,
+             x <> y ->
+             occurs_free_ctx e y ->
+             occurs_free_ctx (Eproj_c x tau n y' e) y
+       | Free_Efun11 :
+           forall y defs e,
+             ~ (name_in_fundefs defs y) -> 
+             occurs_free_ctx e y ->
+             occurs_free_ctx (Efun1_c defs e) y
+       | Free_Efun21 :
+           forall y defs e,
+             ~ (name_in_ctx_fundefs defs y) -> 
+             occurs_free e y ->
+             occurs_free_ctx (Efun2_c defs e) y                             
+       | Free_Efun12 :
+           forall y defs e, 
+             occurs_free_fundefs defs y ->
+             occurs_free_ctx (Efun1_c defs e) y
+       | Free_Efun22 :
+           forall y defs e, 
+             occurs_free_fundefs_ctx defs y ->
+             occurs_free_ctx (Efun2_c defs e) y
+       | Free_Eprim1 :
+           forall y x p ys e,
+             List.In y ys ->
+             occurs_free_ctx (Eprim_c x p ys e) y
+       | Free_Eprim2 :
+           forall y x p ys e,
+             x <> y ->
+             occurs_free_ctx e y ->
+             occurs_free_ctx (Eprim_c x p ys e) y
+       with occurs_free_fundefs_ctx : fundefs_ctx -> Ensemble var :=
+            | Free_Fcons11 :
+                forall x f tau ys e defs,  
+                  x <> f ->
+                  ~ (List.In x ys) ->
+                  ~ (name_in_fundefs defs x) ->
+                  occurs_free_ctx e x ->
+                  occurs_free_fundefs_ctx (Fcons1_c f tau ys e defs) x
+            | Free_Fcons12 :
+                forall x f tau ys e defs,
+                  occurs_free_fundefs defs x ->
+                  x <> f ->
+                  occurs_free_fundefs_ctx (Fcons1_c f tau ys e defs) x
+            | Free_Fcons21 :
+                forall x f tau ys e defs,  
+                  x <> f ->
+                  ~ (List.In x ys) ->
+                  ~ (name_in_ctx_fundefs defs x) ->
+                  occurs_free e x ->
+                  occurs_free_fundefs_ctx (Fcons2_c f tau ys e defs) x
+            | Free_Fcons22 :
+                forall x f tau ys e defs,
+                  occurs_free_fundefs_ctx defs x ->
+                  x <> f ->
+                  occurs_free_fundefs_ctx (Fcons2_c f tau ys e defs) x.
+
+       Hint Constructors occurs_free_ctx occurs_free_fundefs.
+
+       Lemma occurs_free_Econstr_c x t ys e :
+        Same_set var (occurs_free_ctx (Econstr_c x t ys e))
+                 (Union _ (FromList ys) (Setminus var (occurs_free_ctx e) (Singleton var x))).
+      Proof.
+        split; intros x' H; inv H; eauto.
+        right. constructor; eauto. intros H. inv H; eauto.
+        inv H0.  constructor 2; eauto. intros Hc. subst. eauto.
+      Qed.
+
+      Lemma occurs_free_Eprim_c x f ys e :
+        Same_set var (occurs_free_ctx (Eprim_c x f ys e))
+                 (Union _ (FromList ys) (Setminus var (occurs_free_ctx e) (Singleton var x))).
+      Proof.
+        split; intros x' H; inv H; eauto.
+        right. constructor; eauto. intros H. inv H; eauto.
+        inv H0. eapply Free_Eprim2; eauto. intros Hc. subst. eauto.
+      Qed.
+
+       Lemma occurs_free_Eproj_c x tag n y e :
+         Same_set var (occurs_free_ctx (Eproj_c x tag n y e))
+                  (Union _ (Singleton var y) (Setminus var (occurs_free_ctx e) (Singleton var x))).
+       Proof.
+         split; intros x' H; inv H; eauto. 
+         right. constructor; eauto. intros H. inv H; eauto.
+         inv H0. eauto.
+         inv H0. constructor; eauto.
+         intros Hc. subst. eauto.
+       Qed.
+
+       Lemma occurs_free_Efun1_c B e :
+         Same_set var (occurs_free_ctx (Efun1_c B e))
+                  (Union _ (occurs_free_fundefs B)
+                         (Setminus _ (occurs_free_ctx e) (name_in_fundefs B))).
+       Proof.
+         split; intros x' H; inv H; eauto.
+         right; eauto. constructor; eauto.
+         inv H0. eauto. 
+       Qed.
+       
+       Lemma occurs_free_Efun2_c B e :
+         Same_set var (occurs_free_ctx (Efun2_c B e))
+                  (Union _ (occurs_free_fundefs_ctx B)
+                         (Setminus _ (occurs_free e) (name_in_ctx_fundefs B))).
+       Proof.
+         split; intros x' H; inv H; eauto.
+         right; eauto. constructor; eauto.
+         inv H0. eauto. 
+       Qed.
+
+
+       Lemma occurs_free_Ecase_c x cl1 cl2 c e :
+         Same_set var (occurs_free_ctx (Ecase_c x cl1 c e cl2))
+                  (Union _ (Singleton _ x)
+                         (Union _ (occurs_free_ctx e)
+                                (Union _ (occurs_free (Ecase x cl1)) (occurs_free (Ecase x cl2))))).
+       Proof.
+         split; intros x' H; inv H; eauto.
+         inv H0; eauto. inv H0; eauto.
+         inv H; eauto.
+       Qed.
+
+       
+       Lemma occurs_free_fundefs_Fcons1_c f t xs e B :
+         Same_set var (occurs_free_fundefs_ctx (Fcons1_c f t xs e B))
+                  (Union var (Setminus var (occurs_free_ctx e)
+                                       (Union var (Singleton var f)
+                                              (Union var (FromList xs)
+                                                     (name_in_fundefs B))))
+                         (Setminus var (occurs_free_fundefs B) (Singleton var f))).
+       Proof.
+         split; intros x H; inv H.
+         - left. constructor; eauto. intros Hin. inv Hin; eauto.
+           inv H. congruence. inv H; eauto.
+         - right. constructor; eauto. intros H. inv H. congruence.
+         - inv H0. constructor; eauto. 
+           intros Hc. subst. eauto.
+         - inv H0. constructor 2; eauto. intros Hc; subst; eauto.
+       Qed.
+
+       Lemma occurs_free_fundefs_Fcons2_c f t xs e B :
+         Same_set var (occurs_free_fundefs_ctx (Fcons2_c f t xs e B))
+                  (Union var (Setminus var (occurs_free e)
+                                       (Union var (Singleton var f)
+                                              (Union var (FromList xs)
+                                                     (name_in_ctx_fundefs B))))
+                         (Setminus var (occurs_free_fundefs_ctx B) (Singleton var f))).
+       Proof.
+         split; intros x H; inv H.
+         - left. constructor; eauto. intros Hin. inv Hin; eauto.
+           inv H. congruence. inv H; eauto.
+         - right. constructor; eauto. intros H. inv H. congruence.
+         - inv H0. constructor; eauto. 
+           intros Hc. subst. eauto.
+         - inv H0.
+           constructor 4;  eauto.
+           intros Hc; subst; eauto.
+       Qed.
+
+       Lemma occurs_free_Hole_c:
+         Same_set var (occurs_free_ctx Hole_c)
+                  (Empty_set var).
+       Proof.
+         split; intros x H; inv H.
+       Qed.
+
+
+Ltac normalize_occurs_free_ctx :=
+  match goal with
+    | [|- context[occurs_free_ctx (Econstr_c _ _ _ _)]] =>
+      rewrite occurs_free_Econstr_c
+    | [|- context[occurs_free_ctx (Eproj_c _ _ _ _ _)]] =>
+      rewrite occurs_free_Eproj_c
+    | [|- context[occurs_free_ctx (Ecase_c _ _ _ _ _ )]] =>
+      rewrite occurs_free_Ecase_c
+    | [|- context[occurs_free_ctx (Efun1_c _ _)]] =>
+      rewrite occurs_free_Efun1_c
+    | [|- context[occurs_free_ctx (Efun2_c _ _)]] =>
+      rewrite occurs_free_Efun2_c
+    | [|- context[occurs_free_ctx (Eprim_c _ _ _ _)]] =>
+      rewrite occurs_free_Eprim_c
+    | [|- context[occurs_free_fundefs_ctx (Fcons1_c _ _ _ _ _)]] =>
+      rewrite occurs_free_fundefs_Fcons1_c
+    | [|- context[occurs_free_fundefs_ctx (Fcons2_c _ _ _ _ _)]] =>
+      rewrite occurs_free_fundefs_Fcons2_c
+    | [|- context[occurs_free_ctx (Hole_c)]] =>
+      rewrite occurs_free_Hole_c
+  end.
+
+Ltac normalize_occurs_free_ctx_in_ctx :=
+  match goal with
+    | [ H : context[occurs_free_ctx (Econstr_c _ _ _ _)] |- _ ] =>
+      rewrite occurs_free_Econstr_c
+    | [ H : context[occurs_free_ctx (Eproj_c _ _ _ _ _)] |- _ ] =>
+      rewrite occurs_free_Eproj_c
+    | [ H : context[occurs_free_ctx (Ecase_c _ _ _ _ _ )] |- _ ] =>
+      rewrite occurs_free_Ecase_c
+    | [ H : context[occurs_free_ctx (Efun1_c _ _)] |- _ ] =>
+      rewrite occurs_free_Efun1_c
+    | [ H : context[occurs_free_ctx (Efun2_c _ _)] |- _ ] =>
+      rewrite occurs_free_Efun2_c
+    | [ H : context[occurs_free_ctx (Eprim_c _ _ _ _)] |- _ ] =>
+      rewrite occurs_free_Eprim_c
+    | [ H : context[occurs_free_fundefs_ctx (Fcons1_c _ _ _ _ _)] |- _ ] =>
+      rewrite occurs_free_fundefs_Fcons1_c
+    | [ H : context[occurs_free_fundefs_ctx (Fcons2_c _ _ _ _ _)] |- _ ] =>
+      rewrite occurs_free_fundefs_Fcons2_c
+    | [ H : context[occurs_free_ctx (Hole_c)] |- _ ] =>
+      rewrite occurs_free_Hole_c
+  end.
+
+    (* push rename_all_ns and inlined_ctx down *)    
+    Ltac normalize_ctx :=
+      match goal with
+          (* rename_all *)
+        | [H: context[rename_all_ns _ (_ |[ _ ]|)] |- _] =>
+          rewrite (proj1 (rename_all_ns_app_ctx _ _)) in H
+        | [H: context[rename_all_fun_ns _ (_ <[ _ ]>)] |- _] =>
+          rewrite (proj2 (rename_all_ns_app_ctx _ _)) in H
+        | [|- context[rename_all_ns _ (_ |[ _ ]|)]] =>
+          rewrite (proj1 (rename_all_ns_app_ctx _ _))
+        | [|- context[rename_all_fun_ns _ (_ <[ _ ]>)]] =>
+          rewrite (proj2 (rename_all_ns_app_ctx _ _))
+        | [H: context[rename_all_fun_ns _ (fundefs_append _ _)] |- _] =>
+          rewrite rename_all_ns_fundefs_append in H
+        | [|- context[rename_all_fun_ns _ (fundefs_append _ _)]] =>
+          rewrite rename_all_ns_fundefs_append
+        | [H: context[rename_all_ctx_ns _ (comp_ctx_f _ _)] |- _] =>
+          rewrite (proj1 (rename_all_ctx_ns_comp_ctx _ _)) in H
+        | [|- context[rename_all_ctx_ns _ (comp_ctx_f _ _)]] =>
+          rewrite (proj1 (rename_all_ctx_ns_comp_ctx _ _))
+        | [H: context[rename_all_fun_ctx_ns _ (comp_f_ctx_f _ _)] |- _] =>
+          rewrite (proj2 (rename_all_ctx_ns_comp_ctx _ _)) in H
+        | [|- context[rename_all_fun_ctx_ns _ (comp_f_ctx_f _ _)]] =>
+          rewrite (proj2 (rename_all_ctx_ns_comp_ctx _ _))
+
+        (* inlined *)
+        | [H: context[ inlined_ctx_f (comp_ctx_f _ _ ) _ ] |- _] =>
+          rewrite (proj1 (inlined_comp_ctx)) in H
+        | [|-context[ inlined_ctx_f (comp_ctx_f _ _) _]] =>
+          rewrite (proj1 (inlined_comp_ctx))
+        | [H: context[ inlined_fundefs_ctx_f (comp_f_ctx_f _ _) _] |- _] =>
+          rewrite (proj2 (inlined_comp_ctx)) in H
+        | [|-context[ inlined_fundefs_ctx_f (comp_f_ctx_f _ _) _]] =>
+          rewrite (proj2 (inlined_comp_ctx))
+        | [H: context[ inlined_fundefs_f (fundefs_append _ _) _] |- _] =>
+          rewrite inlined_fundefs_append in H
+        | [|-context[ inlined_fundefs_f (fundefs_append _ _) _]] =>
+          rewrite inlined_fundefs_append
+      end.
+
+    Ltac normalize_bound_var_ctx' :=
+      match goal with
+        | [ |- context[bound_var_ctx Hole_c]] =>
+          rewrite bound_var_Hole_c 
+        | [|- context[bound_var_ctx (Econstr_c _ _ _ _)]] =>
+          rewrite bound_var_Econstr_c
+        | [|- context[bound_var_ctx (Eproj_c _ _ _ _ _)]] =>
+          rewrite bound_var_Eproj_c
+        | [|- context[bound_var_ctx (Ecase_c _ _ _ _ _)]] =>
+          rewrite bound_var_Case_c
+        | [ |- context[bound_var_ctx (Efun1_c _ _)]] =>
+          rewrite bound_var_Fun1_c 
+        | [ |- context[bound_var_ctx (Efun2_c _ _)] ] =>
+          rewrite bound_var_Fun2_c
+        | [|- context[bound_var_ctx (Eprim_c _ _ _ _)]] =>
+          rewrite bound_var_Eprim_c
+        | [|- context[bound_var_fundefs_ctx (Fcons1_c _ _ _ _ _)]] =>
+          rewrite bound_var_Fcons1_c
+        | [|- context[bound_var_fundefs_ctx (Fcons2_c _ _ _ _ _)]] =>
+          rewrite bound_var_Fcons2_c
+      end.
+
+Ltac normalize_bound_var_ctx_in_ctx' :=
+  match goal with
+    | [ H: context[bound_var_ctx Hole_c] |- _] =>
+      rewrite bound_var_Hole_c in H
+    | [ H : context[bound_var_ctx (Econstr_c _ _ _ _)] |- _ ] =>
+      rewrite bound_var_Econstr_c in H
+    | [ H : context[bound_var_ctx (Eproj_c _ _ _ _ _)]  |- _ ] =>
+      rewrite bound_var_Eproj_c in H
+    | [H: context[bound_var_ctx (Ecase_c _ _ _ _ _)] |- _] =>
+      rewrite bound_var_Case_c in H
+    | [ H : context[bound_var_ctx (Efun1_c _ _)] |- _ ] =>
+      rewrite bound_var_Fun1_c in H
+    | [ H : context[bound_var_ctx (Efun2_c _ _)] |- _ ] =>
+      rewrite bound_var_Fun2_c in H
+    | [ H : context[bound_var_ctx (Eprim_c _ _ _ _)] |- _ ] =>
+      rewrite bound_var_Eprim_c in H
+    | [H:context[bound_var_fundefs_ctx (Fcons1_c _ _ _ _ _)] |- _] =>
+      rewrite bound_var_Fcons1_c in H
+    | [H: context[bound_var_fundefs_ctx (Fcons2_c _ _ _ _ _)] |- _] =>
+      rewrite bound_var_Fcons2_c in H
+  end.
+
+
+    Theorem bound_var_ctx_comp_ctx:      
+      (forall c1 c2,
+      Same_set _ (bound_var_ctx (comp_ctx_f c1 c2))
+               (Union _ (bound_var_ctx c1) (bound_var_ctx c2)))/\
+      (forall fc1 c2,
+         Same_set _ (bound_var_fundefs_ctx (comp_f_ctx_f fc1 c2))
+               (Union _ (bound_var_fundefs_ctx fc1) (bound_var_ctx c2)))
+       .
+       Proof.
+         exp_fundefs_ctx_induction IHc1 IHfc1; simpl; split; repeat (normalize_bound_var_ctx'); try (rewrite IHc1); try (rewrite IHfc1); repeat (normalize_bound_var_ctx'); repeat (normalize_bound_var); eauto 25 with Ensembles_DB.
+       Qed.
+
+       Ltac  normalize_bound_var_ctx :=
+         first [
+                match goal with
+                  | [|- context[bound_var_ctx (comp_ctx_f _ _)]] =>
+                    rewrite (proj1 (bound_var_ctx_comp_ctx))
+                  | [|- context [bound_var_fundefs_ctx (comp_f_ctx_f _ _)]] =>
+                    rewrite (proj1 (bound_var_ctx_comp_ctx))
+                end | normalize_bound_var_ctx'].
+
+       Ltac  normalize_bound_var_ctx_in_ctx :=
+         first [
+                match goal with
+                  | [H:context[bound_var_ctx (comp_ctx_f _ _)] |- _] =>
+                    rewrite (proj2 (bound_var_ctx_comp_ctx)) in H
+                  | [H:context [bound_var_fundefs_ctx (comp_f_ctx_f _ _)] |- _] =>
+                    rewrite (proj2 (bound_var_ctx_comp_ctx)) in H
+                end| normalize_bound_var_ctx_in_ctx'].
+
+       
+       Definition closed_ctx :=
+          fun c => Empty_set var <--> occurs_free_ctx c.
+         
+       Definition closed_fundefs_ctx :=
+         fun cf => Empty_set var <--> occurs_free_fundefs_ctx cf.
+
+       Definition closed_fundefs :=
+         fun f => Empty_set var <--> occurs_free_fundefs f.
+
+       Theorem Decidable_name_in_ctx_fundefs :
+         forall cf, Decidable (name_in_ctx_fundefs cf).
+       Proof.
+         induction cf; simpl.
+         apply Decidable_Union.
+         apply Decidable_singleton_var.
+         apply Decidable_name_in_fundefs.
+         apply Decidable_Union.
+         apply Decidable_singleton_var.
+         auto.
+       Qed.         
+
+       Theorem fun_names_not_free_in_fundefs_ctx :
+         forall x f7,
+         name_in_ctx_fundefs f7 x
+         -> ~ occurs_free_fundefs_ctx f7 x.
+       Proof.
+         induction f7; intros; intro.
+         inv H; inv H0; auto.
+         inv H1; auto.
+         inv H1; auto.
+         revert H7.
+         apply fun_names_not_free_in_fundefs.
+         auto.
+         inv H; inv H0; auto.
+         inv H1; auto.
+         inv H1; auto.
+         revert H7.
+         apply IHf7; auto.
+       Qed.
+       
+       Theorem occurs_free_ctx_dec :
+         (forall c,
+            Decidable (occurs_free_ctx c)) /\
+         (forall fc,
+            Decidable (occurs_free_fundefs_ctx fc)).
+       Proof.         
+         exp_fundefs_ctx_induction IHc IHf; constructor; intros x; try (inv IHc; specialize (Dec x)); try (inv IHf; specialize (Dec x)).
+         - right; auto.
+           intro. inv H.
+         - assert (Hl := Decidable_FromList l).
+           inv Hl.
+           specialize (Dec0 x).
+           inv Dec0.
+           left; auto.
+           destruct (var_dec  v x).
+           subst.
+           right.
+           intro.
+           inv H0. auto.
+           apply H6; auto.
+           inv Dec.
+           left; auto.
+           right.
+           intro. inv H1; auto.           
+         - destruct (var_dec x v0).
+           subst. left; auto.
+           destruct (var_dec v x).
+           subst.
+           right; intro. inv H; auto.
+           inv Dec.
+           left; auto.
+           right; intro.
+           inv H0; auto.           
+         - assert (Hl := Decidable_FromList l).
+           inv Hl.
+           specialize (Dec0 x).
+           inv Dec0.
+           left; auto.
+           destruct (var_dec  v x).
+           subst.
+           right.
+           intro.
+           inv H0. auto.
+           apply H6; auto.
+           inv Dec.
+           left; auto.
+           right.
+           intro. inv H1; auto.           
+         - assert (Hl := Decidable_occurs_free (Ecase v l)).
+           assert (Hl0 := Decidable_occurs_free (Ecase v l0)).
+           inv Hl. specialize (Dec0 x).
+           inv Hl0. specialize (Dec1 x).
+           inv Dec0.
+           left. apply Free_Ecase3; auto.
+           inv Dec1.
+           left. apply Free_Ecase4; auto.
+           inv Dec.
+           left. constructor; auto.
+           right. intro.
+           inv H2; auto.
+         - assert (Hf4 := Decidable_occurs_free_fundefs f4).
+           inv Hf4; specialize (Dec0 x).
+           inv Dec0.
+           left; auto.
+           assert (Hf4n := Decidable_name_in_fundefs f4).
+           inv Hf4n. specialize (Dec0 x).
+           inv Dec0.
+           right.
+           intro.
+           inv H1; auto.
+           destruct Dec.
+           left; auto.
+           right; intro. inv H2; auto.
+         - assert (He := Decidable_occurs_free e). 
+           inv He; specialize (Dec0 x).
+           inv Dec.
+           left; auto.
+           assert (Hf5 := Decidable_name_in_ctx_fundefs f5).
+           inv Hf5. specialize (Dec x). inv Dec.
+           right.
+           intro; auto. inv H1; auto.
+           inv Dec0.
+           left; auto.
+           right; intro; apply H1.
+           inv H2; auto.
+           exfalso; auto.
+         - destruct (var_dec x v).
+           right.
+           intro. subst. inv H; auto.
+           assert (Hf6 := Decidable_name_in_fundefs f6).
+           inv Hf6. specialize (Dec0 x).
+           inv Dec0.
+           right. intro. inv H0.
+           auto.
+           revert H7; apply fun_names_not_free_in_fundefs; auto.
+           assert (He := Decidable_occurs_free_fundefs f6).
+           inv He. specialize (Dec0 x).
+           inv Dec0.
+           left; constructor 2; auto.
+           inv Dec.
+           assert (Hl := Decidable_FromList l).
+           inv Hl. specialize (Dec x). inv Dec.
+           right; intro; inv H3; auto.
+           left. constructor; auto.
+           right. intro. inv H2; auto.           
+          - destruct (var_dec x v).
+           right.
+           intro. subst. inv H; auto.
+           assert (Hf6 := Decidable_name_in_ctx_fundefs f7).
+           inv Hf6. specialize (Dec0 x).
+           inv Dec0.
+           right. intro. inv H0.
+           auto.
+           revert H7.
+           apply fun_names_not_free_in_fundefs_ctx; auto.
+           inv Dec.
+           left; constructor 4; auto.
+           assert (Hl := Decidable_FromList l).
+           inv Hl. specialize (Dec x). inv Dec.
+           right; intro; inv H2; auto.
+           assert (He :=  Decidable_occurs_free e).
+           inv He. specialize (Dec x). inv Dec. left; constructor; auto.
+           right. intro. inv H3; auto.           
+       Qed.
+
+       Theorem Decidable_occurs_free_ctx:         
+         (forall c,
+            Decidable (occurs_free_ctx c)).
+       Proof.
+         intro; apply occurs_free_ctx_dec; auto.
+       Qed.         
+
+       Theorem Decidable_occurs_free_fundefs_ctx:         
+         forall fc,
+           Decidable (occurs_free_fundefs_ctx fc).
+       Proof.
+         intro; apply occurs_free_ctx_dec; auto.
+       Qed.         
+
+       Lemma occurs_free_included_ctx_mut:
+         forall e,
+           (forall c,
+              Included _ (occurs_free_ctx c) (occurs_free (c|[e]|))) /\
+           (forall fc,
+              Included _ (occurs_free_fundefs_ctx fc) (occurs_free_fundefs (fc <[ e ]>))).
+       Proof.
+         intro e; exp_fundefs_ctx_induction IHc IHf; intros; repeat normalize_occurs_free_ctx; simpl; repeat normalize_occurs_free; eauto with Ensembles_DB.
+         rewrite <- name_in_ctx_fundefs_ctx.
+         eauto with Ensembles_DB.
+         rewrite <- name_in_ctx_fundefs_ctx.
+         eauto with Ensembles_DB.
+       Qed.
+
+
+       Theorem occurs_free_included_ctx:
+               forall e,
+           (forall c,
+              Included _ (occurs_free_ctx c) (occurs_free (c|[e]|))).
+       Proof.
+         intros; apply occurs_free_included_ctx_mut.
+       Qed.
+
+       Theorem occurs_free_included_fundefs_ctx:
+       forall e,
+           (forall fc,
+              Included _ (occurs_free_fundefs_ctx fc) (occurs_free_fundefs (fc <[ e ]>))).
+       Proof.
+         intros; apply occurs_free_included_ctx_mut.
+       Qed.
+
+      Corollary closed_app_ctx:
+         forall e c,
+         closed (c |[ e ]|) ->
+         closed_ctx c. 
+       Proof.
+         intros.
+         assert (Hc := occurs_free_included_ctx e c).
+         apply Included_Empty_set_l.
+         eapply Proper_Included_r; eauto.
+       Qed.
+         
+
+
+
+         
+         
+       Corollary ub_app_ctx_ctx:
+         forall c e v,
+           unique_bindings (c |[ e ]|) ->
+           bound_var_ctx c v ->
+          ~ bound_var e v. 
+       Proof.
+         intros.
+         apply ub_app_ctx_f in H.
+         destructAll.
+         inv H2.
+         specialize (H3 v).
+         intro; apply H3.
+         split; auto.
+       Qed.
+
+       About Decidable_name_in_ctx_fundefs.
+
+       
+(* End move_to_identifiers.*)
+
+       
+       Theorem not_free_dead_or_bound:
+         forall e,
+           Included _ (Complement _ (occurs_free e)) (Union _ (dead_var e) (bound_var e)).
+       Proof.
+         intros.
+         intro. intro.
+         apply not_free_bound_or_not_occur in H.
+         destruct H; auto.
+       Qed.
+
+       Theorem not_bound_dead_or_free:
+         forall e,
+           Included _ (Complement _ (bound_var e)) (Union _ (dead_var e) (occurs_free e)).
+       Proof.
+         intros.
+         intro; intro.
+         assert (He := Decidable_occurs_free e). 
+         inv He. specialize (Dec x).
+         inv Dec; auto.
+         apply not_free_dead_or_bound in H0.
+         inv H0; auto.
+         exfalso. auto.
+       Qed.         
+
+       Theorem closed_sig_inv_dom_implies_sig_inv:
+         forall sig e,
+           closed e ->
+           sig_inv_dom sig e ->
+           sig_inv sig e.
+       Proof.
+         intros.
+         intro; intros.
+         apply H0 in H1.
+         split; auto.
+         assert (~ occurs_free e y). intro.
+         apply H in H2. inv H2.
+         apply not_free_dead_or_bound in H2.
+         inv H2; auto.
+       Qed.
+       
+       Theorem name_in_bound_var_fundefs_ctx: forall cf,
+         Included _ (name_in_ctx_fundefs cf) (bound_var_fundefs_ctx cf).
+       Proof.
+         induction cf; simpl; normalize_bound_var_ctx; auto with Ensembles_DB.
+         intro. intro. inv H. auto.
+         apply name_in_fundefs_bound_var_fundefs in H0.
+         auto.
+       Qed.
+       
+Theorem not_free_bound_or_not_occur_ctx:
+  forall v : var,
+    (forall c : exp_ctx, ~ occurs_free_ctx c v -> num_occur_ec c v 0 \/ bound_var_ctx c v) /\
+    (forall cf : fundefs_ctx,
+       ~ occurs_free_fundefs_ctx cf v -> num_occur_fdc cf v 0 \/ bound_var_fundefs_ctx cf v).
+Proof.
+  intro v; exp_fundefs_ctx_induction IHc IHf; intros; eauto with Ensembles_DB.
+  -  left. constructor.
+  - destruct (var_dec v0 v).
+    + right; subst; auto.
+    + assert (~occurs_free_ctx e v).
+      intro; apply H.
+      constructor 2; auto.
+      apply IHc in H0.
+      inv H0.
+      * left.
+        eapply num_occur_ec_n.
+        constructor. apply H1.
+        assert (~ FromList l v).
+        intro; apply H.
+        auto.
+        apply not_occur_list_not_in in H0. rewrite H0; auto.
+      * right; auto.
+  -  destruct (var_dec v0 v).
+    + right; subst; auto.
+    +  assert (~occurs_free_ctx e v).
+       intro; apply H.
+       auto.
+      apply IHc in H0.
+      inv H0.
+       * left.
+        eapply num_occur_ec_n.
+        constructor. apply H1.
+        simpl. destruct (cps_util.var_dec v v1).
+        subst;
+          exfalso; apply H; auto.
+        auto.
+       * right; auto.
+  -  destruct (var_dec v0 v).
+    + right; subst; auto.
+    +  assert (~occurs_free_ctx e v).
+       intro; apply H.
+       auto.
+      apply IHc in H0.
+      inv H0.
+       * left.
+        eapply num_occur_ec_n.
+        constructor. apply H1.
+        simpl.
+        assert (~ FromList l v).
+        intro; apply H.
+        auto.
+        apply not_occur_list_not_in in H0. rewrite H0; auto.
+      * right; auto.
+  - assert (~ Union var [set v0]
+          (Union var (occurs_free_ctx e)
+             (Union var (occurs_free (Ecase v0 l))
+                    (occurs_free (Ecase v0 l0)))) v).
+    intro. apply H.
+    apply occurs_free_Ecase_c.
+    auto.
+    assert (v <> v0).
+    intro; apply H0; subst; 
+    left; auto.
+    assert (~ occurs_free (Ecase v0 l) v).
+    intro; apply H0.
+    right; right; left; auto.
+    assert (~ occurs_free (Ecase v0 l0) v).
+    intro; apply H0.
+    right; right; right; auto.
+    assert (~(occurs_free_ctx e) v). 
+    intro; apply H0.
+    right; left; auto.
+    clear H0.
+    apply IHc in H4.
+    apply not_free_bound_or_not_occur in H2.
+    apply not_free_bound_or_not_occur in H3. 
+    destruct H2.
+    destruct H3.
+    destruct H4.
+    left.
+    inv H0; pi0.
+    inv H2; pi0.
+    eapply num_occur_ec_n.
+    constructor; eauto.
+    simpl. destruct (cps_util.var_dec v v0). subst; exfalso; auto.
+    auto.
+    right; auto.
+    right; auto.
+    inv H2.
+    eapply Bound_Case3_c; eauto.
+    right.
+    inv H0;
+    eapply Bound_Case2_c; eauto.
+  - assert (Hf4 := Decidable_name_in_fundefs f4).
+    destruct Hf4.
+    specialize (Dec v).
+    inv Dec.
+    right.
+    constructor.
+    apply name_in_fundefs_bound_var_fundefs.
+    auto.
+    assert (~ occurs_free_ctx e v).
+    intro; apply H; auto.
+    assert (~ occurs_free_fundefs f4 v).
+    intro; apply H. auto.
+    apply IHc in H1.
+    apply not_free_bound_or_not_occur in H2.
+    destruct H1.
+    destruct H2.
+    left.
+    eapply num_occur_ec_n.
+    constructor; eauto.
+    auto.
+    right; auto.
+    right; auto.
+  - assert (Hf5 := Decidable_name_in_ctx_fundefs f5).
+    destruct Hf5.
+    specialize (Dec v).
+    inv Dec.
+    right.
+    constructor.
+    apply name_in_bound_var_fundefs_ctx. auto.
+    assert (~ occurs_free_fundefs_ctx f5 v).
+    intro; apply H; auto.
+    assert (~ occurs_free e v).
+    intro; apply H; auto.
+    apply IHf in H1.
+    apply not_free_bound_or_not_occur in H2.
+    inv H1. inv H2.
+    left.
+    eapply num_occur_ec_n.
+    constructor; eauto. auto.
+    right; auto.
+    right; auto.
+  - destruct (var_dec v0 v).
+    right; subst.
+    constructor.
+    assert (Hl := Decidable_FromList l).
+    inv Hl.
+    specialize (Dec v).
+    inv Dec.
+    right; auto.
+    assert (Hf6 := Decidable_name_in_fundefs f6).
+    destruct Hf6.
+    specialize (Dec v).
+    inv Dec.
+    right. apply name_in_fundefs_bound_var_fundefs in H1. auto.
+    assert (~ occurs_free_ctx e v).
+    intro; apply H.
+    constructor; auto.
+    apply IHc in H2.
+    assert (~ occurs_free_fundefs f6 v).
+    intro; apply H. constructor 2; auto.
+    apply not_free_bound_or_not_occur in H3. 
+    inv H2.
+    inv H3.
+    left. eapply num_occur_fdc_n.
+    constructor; eauto. auto.
+    right. auto.
+    right. auto.    
+  - destruct (var_dec v0 v).
+    right; subst.
+    constructor.
+    assert (Hl := Decidable_FromList l).
+    inv Hl.
+    specialize (Dec v).
+    inv Dec.
+    right; auto.
+    assert (Hf7 := Decidable_name_in_ctx_fundefs f7).
+    destruct Hf7.
+    specialize (Dec v).
+    inv Dec.
+    right. apply name_in_bound_var_fundefs_ctx in H1. auto.
+    assert (~ occurs_free e v).
+    intro; apply H.
+    constructor; auto.
+    apply not_free_bound_or_not_occur in H2. 
+    assert (~ occurs_free_fundefs_ctx f7 v).
+    intro; apply H. apply Free_Fcons22; auto.
+    apply IHf in H3.
+    inv H2.
+    inv H3.
+    left. eapply num_occur_fdc_n.
+    constructor; eauto. auto.
+    right. auto.
+    right. auto.
+Qed.
+
+
+
+
+       Theorem not_free_dead_or_bound_ctx:
+         forall c,
+           Included _ (Complement _ (occurs_free_ctx c)) (Union _ (dead_var_ctx c) (bound_var_ctx c)).
+       Proof.
+         intros.
+         intro. intro.
+         apply not_free_bound_or_not_occur_ctx in H.
+         destruct H; auto.
+       Qed.
+
+       
+              Theorem not_bound_dead_or_free_ctx:
+         forall e,
+           Included _ (Complement _ (bound_var_ctx e)) (Union _ (dead_var_ctx e) (occurs_free_ctx e)).
+       Proof.
+         intros.
+         intro; intro.
+         assert (He := (proj1 occurs_free_ctx_dec) e).
+         inv He. specialize (Dec x).
+         inv Dec; auto.
+         apply not_free_dead_or_bound_ctx in H0.
+         inv H0; auto.
+         exfalso. auto.
+       Qed.         
+
+       
+
+
+       Theorem closed_not_occurs_in_context:
+         forall c v,
+           closed_ctx c ->
+           ~ bound_var_ctx c v ->
+           num_occur_ec c v 0.
+       Proof.
+         intros.
+         assert (~ occurs_free_ctx c v).
+         intro.
+         apply H in H1.
+         inv H1.
+         apply not_free_bound_or_not_occur_ctx in H1.
+         inv H1; auto.
+         exfalso; auto.
+       Qed.
+
+       
+        
+    Theorem closed_implies_Disjoint:
+      forall e,
+      closed e ->
+      Disjoint _ (bound_var e) (occurs_free e).
+    Proof.
+      intros. split; intro. intro.
+      inv H0.
+      apply H in H2. inv H2.
+    Qed.
+
+
+    (* if closed at top level, then any subterm is Disjoint OF BV *)
+ (* not used 
+    Theorem closed_app_fun_not_occurs:
+      forall c fds y e',
+      bound_var_fundefs fds y ->
+      ~ name_in_fundefs fds y ->
+      closed (c |[ Efun fds e' ]|) ->
+      unique_bindings (c |[ Efun fds e' ]|) ->
+      num_occur (c |[ e' ]|) y 0.
+    Proof.
+      intros.
+      assert (~ bound_var_ctx c y).
+      apply ub_app_ctx_f in H2.
+      destructAll.
+      intro.
+      inv H4.
+      specialize (H6 y).
+      apply H6. split; auto.
+      assert (num_occur_ec c y 0).
+      apply closed_app_ctx in H1.
+      assert (~ occurs_free_ctx c y).
+      intro.
+      apply H1 in H4.
+      inv H4.
+      apply not_free_dead_or_bound_ctx in H4.
+      inv H4; auto.
+      exfalso; auto.
+      assert (~ bound_var e' y).
+      intro.
+      apply ub_app_ctx_f in H2.
+      destructAll.
+      inv H6.
+      inv H12. specialize (H6 y); apply H6; auto.
+      assert (num_occur e' y 0).
+      {
+        apply not_bound_dead_or_free in H5.
+        inv H5; auto.
+        exfalso.
+        admit.
+      }
+      apply num_occur_app_ctx; eauto.
+    Admitted.      
+*)
+    
+    Theorem gsr_preserves_sig_dom:
+      forall sig ce ce',
+        unique_bindings ce ->
+        closed ce ->
+        gsr_clos ce ce' ->
+        sig_inv_dom sig ce ->
+        sig_inv_dom sig ce'. 
+    Proof.      
+      intros sig ce ce' Hub Hdj H H0.
+      induction H; auto.
+      inv H. intro.
+      intros.
+
+      apply H0 in H.
+      inv H1.
+      (* dead var *)
+      - intro;
+        apply H.
+          apply bound_var_app_ctx in H1.
+          apply bound_var_app_ctx.
+          normalize_bound_var.
+          destruct H1; auto.
+      -   intro.
+          apply H.
+          apply bound_var_app_ctx in H1.
+          apply bound_var_app_ctx.
+          normalize_bound_var.
+          destruct H1; auto.
+      - intro.
+          apply H.
+          apply bound_var_app_ctx in H1.
+          apply bound_var_app_ctx.
+          normalize_bound_var.
+          destruct H1; auto.
+      - intro.
+        apply H.
+          apply bound_var_app_ctx in H1.
+          apply bound_var_app_ctx.
+          normalize_bound_var.
+          destruct H1; auto.
+       - intro.
+          apply H.
+          apply bound_var_app_ctx in H1.
+          apply bound_var_app_ctx.          
+          normalize_bound_var.
+          rewrite bound_var_Efun in H1.
+          rewrite fundefs_append_bound_vars.
+          2: reflexivity.
+          rewrite fundefs_append_bound_vars in H1.
+          2: reflexivity.
+          rewrite bound_var_fundefs_Fcons.          
+          destruct H1; auto.
+          destruct H1; auto.
+          destruct H1; auto.
+          right. left. right.
+          auto.
+        (* fold *)
+      -  intro.
+          apply H.
+          apply bound_var_app_ctx.
+          apply bound_var_app_ctx in H1. destruct H1; auto.
+          right.
+          rewrite bound_var_Econstr in *.
+          destruct H1; auto.
+          left.
+          apply bound_var_app_ctx.
+          apply bound_var_app_ctx in H1. destruct H1; auto.
+          right.
+          eapply Bound_Ecase. apply H1.
+          apply findtag_In_patterns. eauto.
+      -  intro.
+          apply H.
+          apply bound_var_app_ctx.
+          apply bound_var_app_ctx in H1. destruct H1; auto.
+          right.
+          rewrite bound_var_Econstr in *.
+          destruct H1; auto.
+          left.
+          apply bound_var_app_ctx.
+          apply bound_var_app_ctx in H1. destruct H1; auto.
+          right.
+          rewrite bound_var_Eproj.
+          left.
+          unfold rename in H1.
+          apply bound_var_rename_all_exp in H1.
+          auto.
+      (* inline *)
+      -  intro.
+          apply H.
+          apply bound_var_app_ctx.
+          apply bound_var_app_ctx in H1.
+          inv H1; auto.
+          right.
+          rewrite bound_var_Efun.
+          rewrite bound_var_Efun in H4.
+          rewrite fundefs_append_bound_vars.
+          2: reflexivity.
+          rewrite fundefs_append_bound_vars in H4.
+          2: reflexivity.
+          rewrite bound_var_fundefs_Fcons.
+          inv H4; auto.
+          left.
+          inv H1; auto.
+          apply bound_var_app_ctx in H1.
+          inv H1.
+          right.
+          apply bound_var_app_ctx.
+          auto.
+          apply bound_var_rename_all in H4.
+          left.
+          auto.
+      - apply gsr_preserves_clos in H; auto. destruct H.
+        apply gsr_preserves_clos in H1; auto.         
+    Qed.
+
+    Theorem gsr_preserves_sig:
+      forall sig ce ce',
+        unique_bindings ce ->
+        closed ce ->
+        gsr_clos ce ce' ->
+        sig_inv sig ce ->
+        sig_inv sig ce'. 
+    Proof.
+      intros.
+      apply sig_inv_implies_dom in H2.
+      assert (He' := gsr_preserves_clos _ _ H H0 H1).
+      destruct He'.
+      apply closed_sig_inv_dom_implies_sig_inv; auto.
+      eapply gsr_preserves_sig_dom.
+      apply H.
+      auto. auto. auto.
+    Qed.
+
+
+    (* todo: replace shrink_cps_correct's def with that *)
+ Definition eq_env_P {A}:  Ensemble var -> M.t A -> M.t A -> Prop :=
+    fun S rho1 rho2 =>
+      forall x, S x -> M.get x rho1 = M.get x rho2.
+
+
+ Theorem eq_P_apply_r:
+   forall x sub sub',
+   eq_env_P (Singleton _ x) sub sub' ->
+   apply_r sub x = apply_r sub' x.
+ Proof.
+   intros.
+   unfold apply_r.   
+   rewrite H.
+   auto.
+   constructor.
+ Qed.
+   
+ Theorem eq_P_apply_r_list:
+   forall sub sub' l,
+   eq_env_P (FromList l) sub sub' ->
+   apply_r_list sub l = apply_r_list sub' l.
+ Proof.
+   induction l.
+   auto.
+   simpl.
+   intros.
+   erewrite eq_P_apply_r.
+   erewrite IHl. auto.
+   intro. intro. apply H.
+   constructor 2; auto.
+   intro. intro; apply H.
+   constructor.
+   inv H0. auto.
+ Qed.
+ 
+    Theorem eq_P_rename_all_ns :
+      (forall e : exp,
+       forall sub sub' : maps_util.M.t var,
+         eq_env_P (Complement _ (dead_var e)) sub sub' ->
+         rename_all_ns sub e = rename_all_ns sub' e) /\
+      (forall fds : fundefs,
+         forall sub sub' : maps_util.M.t var,
+ eq_env_P (Complement _ (dead_var_fundefs fds)) sub sub' ->
+         rename_all_fun_ns sub fds = rename_all_fun_ns sub' fds).
+    Proof.
+      apply exp_def_mutual_ind; intros; simpl.
+      - erewrite H.
+        Focus 2.
+        intro. intro. apply H0.
+        intro. apply H1. inv H2; pi0; auto.
+        erewrite eq_P_apply_r_list.
+        reflexivity.
+        intro; intro; apply H0.
+        intro. inv H2.
+        pi0.
+        apply not_occur_list in H3.
+        auto.
+      - erewrite eq_P_apply_r.
+        auto.
+        intro; intro; apply H.
+        inv H0.
+        intro. inv H0.
+        destruct (cps_util.var_dec x x).
+        inv H5.
+        apply n0; auto.
+      - erewrite H.
+        assert  (eq_env_P (Complement var (dead_var (Ecase v l))) sub sub').
+        intro; intro; apply H1; intro.
+        inv H3; pi0; auto. inv H7; pi0; auto.
+        apply H2. eapply num_occur_n.
+        constructor; eauto.
+        simpl. destruct (cps_util.var_dec x v); auto.
+        exfalso; auto.
+        apply H0 in H2. simpl in H2. inv H2.
+        auto.
+        intro; intro; apply H1; intro.
+        inv H3. inv H7; pi0.
+        auto.
+      - erewrite eq_P_apply_r.
+        erewrite H.
+        reflexivity.
+        intro; intro; apply H0.
+        intro. inv H2. pi0; auto.
+        intro; intro. apply H0.
+        intro. inv H2. pi0; auto.
+        inv H1.
+        auto.
+      - erewrite H. erewrite H0.
+        auto.
+        intro; intro; apply H1.
+        intro. inv H3; pi0; auto.
+        intro; intro; apply H1.
+        intro. inv H3; pi0; auto.
+      - erewrite eq_P_apply_r.
+        erewrite eq_P_apply_r_list.
+        reflexivity.
+        intro; intro. apply H. intro. inv H1; pi0.
+        apply not_occur_list in H2.
+        auto.
+        intro; intro. apply H. intro.
+        inv H0; inv H1; auto.
+        pi0.
+      - erewrite H.
+        Focus 2.
+        intro. intro. apply H0.
+        intro. apply H1. inv H2; pi0; auto.
+        erewrite eq_P_apply_r_list.
+        reflexivity.
+        intro; intro; apply H0.
+        intro. inv H2.
+        pi0.
+        apply not_occur_list in H3.
+        auto.
+      - erewrite eq_P_apply_r.
+        auto.
+        intro; intro; apply H; intro.
+        inv H0. inv H1; pi0.
+      - erewrite H.
+        erewrite H0; auto.
+        intro; intro; apply H1; intro.
+        inv H3; pi0; auto.
+        intro; intro; apply H1; intro.
+        inv H3; pi0; auto.
+      - auto.
+    Qed.
+
+    Theorem eq_P_rename_all_ctx_ns :
+      (forall e : exp_ctx,
+       forall sub sub' : maps_util.M.t var,
+         eq_env_P (Complement _ (dead_var_ctx e)) sub sub' ->
+         rename_all_ctx_ns sub e = rename_all_ctx_ns sub' e) /\
+      (forall fds : fundefs_ctx,
+         forall sub sub' : maps_util.M.t var,
+ eq_env_P (Complement _ (dead_var_fundefs_ctx fds)) sub sub' ->
+         rename_all_fun_ctx_ns sub fds = rename_all_fun_ctx_ns sub' fds).
+    Proof.
+      exp_fundefs_ctx_induction IHc IHfdc; intros; simpl; auto.
+      - erewrite IHc.
+        erewrite eq_P_apply_r_list.
+        auto.
+        intro; intro; apply H; intro.
+        inv H1; pi0.
+        apply not_occur_list in H1. auto.
+        intro; intro; apply H; intro.
+        inv H1; pi0. auto.
+      - erewrite IHc.
+        erewrite eq_P_apply_r.
+        auto.
+        intro; intro; apply H; intro; inv H1; pi0. inv H0; auto.
+        intro; intro; apply H; intro; inv H1; pi0; auto.
+      - erewrite IHc.
+        erewrite eq_P_apply_r_list.
+        auto.
+        intro; intro; apply H; intro.
+        inv H1; pi0.
+        apply not_occur_list in H1. auto.
+        intro; intro; apply H; intro.
+        inv H1; pi0. auto.
+      - assert (rename_all_ns sub (Ecase v l) = rename_all_ns sub' (Ecase v l)).
+        erewrite (proj1 eq_P_rename_all_ns).
+        reflexivity.
+        intro; intro; apply H; intro. inv H1; pi0. apply H0.
+        eapply num_occur_n.
+        constructor; eauto.
+        simpl. destruct (cps_util.var_dec x v); eauto. exfalso; auto.
+        assert (rename_all_ns sub (Ecase v l0) = rename_all_ns sub' (Ecase v l0)).
+        erewrite (proj1 eq_P_rename_all_ns).
+        reflexivity.
+        intro; intro; apply H; intro. inv H2; pi0. apply H1.
+        eapply num_occur_n.
+        constructor; eauto.
+        simpl. destruct (cps_util.var_dec x v); eauto. exfalso; auto.
+        simpl in *. inv H0; inv H1.
+        erewrite IHc. reflexivity.
+        intro; intro; apply H; intro.
+        inv H1; pi0; auto.        
+      - erewrite IHc.
+        erewrite (proj2 eq_P_rename_all_ns).
+        auto.
+        intro; intro; apply H; intro; inv H1; pi0; auto.
+        intro; intro; apply H; intro; inv H1; pi0; auto.
+      - erewrite IHfdc.
+        erewrite (proj1 eq_P_rename_all_ns).
+        auto.
+        intro; intro; apply H; intro; inv H1; pi0; auto.
+        intro; intro; apply H; intro; inv H1; pi0; auto.
+      - erewrite IHc.
+        erewrite (proj2 eq_P_rename_all_ns).
+        auto.
+        intro; intro; apply H; intro; inv H1; pi0; auto.
+        intro; intro; apply H; intro; inv H1; pi0; auto.
+      - erewrite IHfdc.
+        erewrite (proj1 eq_P_rename_all_ns).
+        auto.
+        intro; intro; apply H; intro; inv H1; pi0; auto.
+        intro; intro; apply H; intro; inv H1; pi0; auto.
+    Qed.
+        
+    (* todo: move to ctx *)
+
+
+      
+    Theorem cmap_view_case:
+      forall sub c x cl1 c0 cl2,
+      cmap_view_ctx sub c -> 
+        cmap_view_ctx sub (comp_ctx_f c (Ecase_c x cl1 c0 Hole_c cl2)).
+    Proof.
+      intros.
+      split; intros; split; intros.
+      - apply H in H0.
+        destructAll.
+        eexists; eexists; eauto.
+        rewrite comp_ctx_f_assoc.
+        simpl.
+        reflexivity.
+      - destructAll.
+        destruct H.
+        apply H.
+        exists x1.
+        apply comp_ctx_split in H0.
+        destruct H0.
+        + destructAll.
+          destruct x3; inv H0.
+          eexists; eauto.
+        + destructAll.
+          destruct x4; inv H3.
+          destruct x4; inv H6.
+      - apply H in H0.
+        destructAll.
+        eexists; eexists; eexists; eexists.
+        rewrite comp_ctx_f_assoc.
+        simpl.
+        reflexivity.
+      - destructAll.
+        destruct H.
+        apply H1.
+        exists x0.
+        apply comp_ctx_split in H0.
+        destruct H0.
+        + destructAll.
+          destruct x4; inv H0.
+          exists x4, x2, x3; auto.
+        + destructAll.
+          destruct x5; inv H3.
+          destruct x5; inv H6.
+    Qed.
+
+    
+    Fixpoint fundefs_ctx_append B1 B2:=
+      match B1 with
+        | Fcons f t xs xe B => Fcons2_c f t xs xe (fundefs_ctx_append B B2)
+        | Fnil => B2
+      end.
+
+    Print comp_f_ctx_f.
+    
+    Theorem fundex_ctx_comp_f_ctx:
+      forall fds1 f1 c v f l fds2,
+       fundefs_ctx_append fds1 (Fcons1_c v f l Hole_c fds2) =
+       comp_f_ctx_f f1 c ->
+       c = Hole_c.
+    Proof.
+      induction fds1; intros.
+      -  simpl in H.
+         destruct f1; inv H.
+         apply IHfds1 in H5. auto.
+      - simpl in H.
+        destruct f1; inv H.
+        destruct e; inv H4. simpl; auto.
+    Qed.
+    
+    Theorem cmap_view_efun2:
+      forall sub c fds1 fds2 v f l e,
+      cmap_view_ctx sub c -> 
+      cmap_view_ctx sub
+                    (comp_ctx_f c
+                                (Efun2_c (fundefs_ctx_append fds1                                  
+                                                             (Fcons1_c v f l Hole_c fds2)) e)).
+    Proof.
+      intros. split; intros; split; intros.
+      - apply H in H0.
+        destructAll.
+        exists x0.
+        exists (comp_ctx_f x1 (Efun2_c (fundefs_ctx_append fds1 (Fcons1_c v f l Hole_c fds2)) e)).
+        rewrite comp_ctx_f_assoc.
+        simpl. auto.
+      - apply H.
+        destructAll.
+        apply comp_ctx_split in H0.
+        destruct H0.
+        + destructAll.
+          destruct x2; inv H0.
+          eauto.
+        + destructAll.
+          destruct x3; inv H2.
+          apply fundex_ctx_comp_f_ctx in H1.
+          inv H1.
+      - apply H in H0.
+        destructAll.
+        exists x.
+        exists (comp_ctx_f x0 (Efun2_c (fundefs_ctx_append fds1 (Fcons1_c v f l Hole_c fds2)) e)).
+        exists x1, x2.
+        rewrite comp_ctx_f_assoc.
+        auto. 
+      - apply H.
+        destructAll.
+        apply comp_ctx_split in H0.
+        destruct H0.
+        + destructAll.
+          destruct x3; inv H0.
+          eauto.
+        + destructAll.
+          destruct x4; inv H2.
+          apply fundex_ctx_comp_f_ctx in H1.
+          inv H1.
+    Qed.      
+
+   
+    Theorem cmap_view_constr:
+    forall {sub c} x t xs, 
+      cmap_view_ctx sub c ->
+      M.get x sub = None ->
+    cmap_view_ctx (M.set x (SVconstr t xs) sub) (comp_ctx_f c (Econstr_c x t xs Hole_c)).
+    Proof.
+      intros; split; intros; split; intros.
+      - destruct (var_dec x0 x).
+        + exists c, Hole_c.
+          subst.
+          rewrite M.gss in H1. inv H1. auto.
+        + rewrite M.gso in H1 by auto.
+          apply H in H1.
+          destructAll.
+          exists x1, (comp_ctx_f x2 (Econstr_c x t xs Hole_c)).
+          rewrite comp_ctx_f_assoc.
+          simpl. auto.
+      - destructAll.
+        apply comp_ctx_split in H1.
+        destruct H1.
+        + destructAll.
+          destruct x3; inv H1.
+          * rewrite M.gss. auto.
+          * rewrite M.gso.
+            Focus 2.
+            intro.
+            subst.
+            destruct H. specialize (H x c l).
+            assert ((exists c' c'' : exp_ctx,
+         comp_ctx_f x1 (Econstr_c x c l x3) =
+         comp_ctx_f c' (Econstr_c x c l c''))) by eauto.
+            apply H in H2. rewrite H0 in H2. inv H2.
+            apply H. eauto.
+        + destructAll.
+          destruct x4; inv H3.
+          * rewrite M.gss; auto.
+          * destruct x4; inv H6.
+      - rewrite M.gso in H1.
+        apply H in H1. destructAll.
+        exists x0.
+        exists (comp_ctx_f x1 (Econstr_c x t xs Hole_c)).
+        rewrite comp_ctx_f_assoc. simpl. eauto.
+        intro.
+        subst.
+        rewrite M.gss in H1. inv H1.
+      - destructAll.
+        rewrite M.gso.
+        apply H.
+        apply comp_ctx_split in H1.
+        destruct H1.
+        + destructAll; subst.
+          destruct x4; inv H1.
+          eauto.
+        + destructAll. destruct x5; inv H3.
+          destruct x5; inv H6.
+        + intro; subst.
+          apply comp_ctx_split in H1.
+          destruct H1.
+          * destructAll; subst.
+            destruct x4; inv H1.
+            destruct H.
+            specialize (H1 x t0 ys e).
+            assert
+              (exists (c' c'' : exp_ctx) (B1 B2 : fundefs),
+          comp_ctx_f x0 (Efun1_c (fundefs_append x2 (Fcons x t0 ys e x3)) x4) =
+          comp_ctx_f c' (Efun1_c (fundefs_append B1 (Fcons x t0 ys e B2)) c'')) by eauto.
+            apply H1 in H2. rewrite H0 in H2. inv H2.
+          * destructAll.
+            destruct x5; inv H3.
+            destruct x5; inv H6.
+    Qed.
+
+    Theorem cmap_view_prim:
+      forall sub c v p l,
+      cmap_view_ctx sub c ->
+      cmap_view_ctx sub (comp_ctx_f c (Eprim_c v p l Hole_c)).
+    Proof.    
+      intros; split; intros; split; intros.
+      - apply H in H0.
+        destructAll.
+        eexists; eexists.
+        rewrite  comp_ctx_f_assoc.
+        simpl. reflexivity.
+      - apply H. destructAll.
+        apply comp_ctx_split in H0.
+        destruct H0; destructAll.
+        + destruct x2; inv H0.
+          eauto.
+        + destruct x3; inv H2.
+          destruct x3; inv H5.
+      - apply H in H0.
+        destructAll.
+        eexists; eexists; eexists; eexists.
+        rewrite  comp_ctx_f_assoc.
+        simpl. reflexivity.
+      - apply H.
+        destructAll.
+        apply comp_ctx_split in H0.
+        destruct H0; destructAll.
+        + destruct x3; inv H0.
+          eauto.
+        + destruct x4; inv H2.
+          destruct x4; inv H5.
+    Qed.
+
+    Theorem cmap_view_proj:
+      forall sub c v t n v',
+      cmap_view_ctx sub c ->
+      cmap_view_ctx sub (comp_ctx_f c (Eproj_c v t n v' Hole_c)).
+    Proof.    
+      intros; split; intros; split; intros.
+      - apply H in H0.
+        destructAll.
+        eexists; eexists.
+        rewrite  comp_ctx_f_assoc.
+        simpl. reflexivity.
+      - apply H. destructAll.
+        apply comp_ctx_split in H0.
+        destruct H0; destructAll.
+        + destruct x2; inv H0.
+          eauto.
+        + destruct x3; inv H2.
+          destruct x3; inv H6.
+      - apply H in H0.
+        destructAll.
+        eexists; eexists; eexists; eexists.
+        rewrite  comp_ctx_f_assoc.
+        simpl. reflexivity.
+      - apply H.
+        destructAll.
+        apply comp_ctx_split in H0.
+        destruct H0; destructAll.
+        + destruct x3; inv H0.
+          eauto.
+        + destruct x4; inv H2.
+          destruct x4; inv H6.
+    Qed.
+
+    
+    Theorem cmap_view_efun1_cons:
+    forall c0 c f0 v f l e,
+    cmap_view_ctx c0 (comp_ctx_f c (Efun1_c f0 Hole_c)) ->
+    M.get v c0 = None -> 
+    cmap_view_ctx (M.set v (SVfun f l e) c0)
+                  (comp_ctx_f c (Efun1_c (Fcons v f l e f0) Hole_c)).
+    Proof.
+      intros; split; intros; split; intros.
+      - rewrite M.gso in H1. apply H in H1.
+        destructAll.
+        apply comp_ctx_split in H1. destruct H1.
+        + destructAll. destruct x2; inv H1.
+          exists x0, (comp_ctx_f x2 (Efun1_c (Fcons v f l e f0) Hole_c)).
+          rewrite comp_ctx_f_assoc. auto.
+        + destructAll.
+          destruct x3; inv H3.
+          destruct x3; inv H4.
+        + intro. subst.
+          rewrite M.gss in H1.
+          inv H1.
+      - destructAll.
+        rewrite M.gso.
+        apply H.
+        apply comp_ctx_split in H1.
+        destruct H1.
+        + destructAll.
+          destruct x2; inv H1.
+          exists x0, (comp_ctx_f x2 (Efun1_c f0 Hole_c)).
+          rewrite comp_ctx_f_assoc. auto.
+        + destructAll.
+          destruct x3; inv H3.
+          destruct x3; inv H4.
+        + intro; subst.
+          apply comp_ctx_split in H1.
+          destruct H1.
+          * destructAll. 
+            destruct x; inv H1.
+            assert (exists e e', (comp_ctx_f (comp_ctx_f x0 (Econstr_c v0 c l0 x)) (Efun1_c f0 Hole_c)) = (comp_ctx_f e (Econstr_c v0 c l0 e'))).
+            exists x0, (comp_ctx_f x (Efun1_c f0 Hole_c)).
+            rewrite comp_ctx_f_assoc.
+            auto.
+            apply H in H1.
+            rewrite H0 in H1. inv H1.
+          * destructAll. destruct x2; inv H3.
+            destruct x2; inv H4.
+      - destruct (var_dec f1 v).
+        + subst. rewrite M.gss in H1.
+          inv H1.
+          exists  c, Hole_c, Fnil, f0.
+          simpl. auto.
+        + rewrite M.gso in H1 by auto.
+          apply H in H1. destructAll.
+          apply comp_ctx_split in H1.
+          destruct H1.
+          * destructAll.
+            destruct x3; inv H1.
+            exists  (comp_ctx_f x Hole_c), Hole_c, (Fcons v f l e x1), x2.
+            auto.
+            exists x, (comp_ctx_f x3 (Efun1_c (Fcons v f l e f0) Hole_c)), x1, x2.
+            rewrite comp_ctx_f_assoc. auto.
+          * destructAll.
+            destruct x4; inv H3.
+            exists x3, Hole_c, (Fcons v f l e x1), x2. auto.
+            destruct x4; inv H4.
+      - destructAll.
+        apply comp_ctx_split in H1.
+        destruct H1.
+        + destructAll.
+          destruct x3; inv H1.
+          * destruct x1; inv H3.
+            rewrite M.gso.
+            apply H. exists (comp_ctx_f x Hole_c), Hole_c, x1, x2.
+            auto.
+            intro; subst.
+            assert (exists g1 g2 B1 B2, (comp_ctx_f (comp_ctx_f x Hole_c)
+                                              (Efun1_c (fundefs_append x1 (Fcons v t ys e0 x2)) Hole_c)) =
+                                        comp_ctx_f g1 (Efun1_c (fundefs_append B1 (Fcons v t ys e0 B2)) g2)).
+            eauto.
+            apply H in H1. rewrite H0 in H1. inv H1.
+            rewrite M.gss. auto.
+          * assert (M.get f1 c0 = Some (SVfun t ys e0)).
+            apply H.
+            exists x, (comp_ctx_f x3 (Efun1_c f0 Hole_c)), x1, x2.
+            rewrite comp_ctx_f_assoc.
+            auto.
+            destruct (var_dec f1 v).
+            subst.
+            rewrite H1 in H0.
+            inv H0.
+            rewrite M.gso; auto.
+        + destructAll.
+          destruct x4; inv H3.
+          * destruct x1; inv H2.
+            assert (M.get f1 c0 = Some (SVfun t ys e0)).
+            apply H.
+            exists x3, Hole_c, x1, x2.
+            auto.
+            destruct (var_dec f1 v0).
+            subst. rewrite H1 in H0. inv H0.
+            rewrite M.gso; auto.
+            rewrite M.gss. auto.
+          * destruct x4; inv H4.
+    Qed.
+            
+    Theorem cmap_view_efun1_nil:
+      forall sub c,
+      cmap_view_ctx sub c ->
+      cmap_view_ctx sub (comp_ctx_f c (Efun1_c Fnil Hole_c)).
+    Proof.
+      intros. split; intros; split; intros.
+      - apply H in H0.
+        destructAll.
+        eexists x0, (comp_ctx_f x1 (Efun1_c Fnil Hole_c)).
+        rewrite comp_ctx_f_assoc. auto.
+      - apply H. destructAll.
+        apply comp_ctx_split in H0.
+        destruct H0.
+        + destructAll. destruct x2; inv H0.
+          eauto.
+        + destructAll. destruct x3; inv H2. destruct x3; inv H3.
+      - apply H in H0.
+        destructAll.
+        exists x, (comp_ctx_f x0 (Efun1_c Fnil Hole_c)), x1, x2.
+        rewrite comp_ctx_f_assoc; auto.
+      - apply H. destructAll.
+        apply comp_ctx_split in H0.
+        destruct H0.
+        + destructAll.
+          destruct x3; inv H0.
+          * destruct x1; inv H2.
+          * eauto.
+        + destructAll.
+          destruct x4; inv H2.
+          destruct x1; inv H1.
+          destruct x4; inv H3.
+    Qed.
+          
+
+       Theorem bound_var_ctx_rename_all_ns:
+               forall sigma, 
+                 (forall (c : exp_ctx),
+                    bound_var_ctx c <--> bound_var_ctx (rename_all_ctx_ns sigma c)) /\
+                 (forall (fdc : fundefs_ctx),
+                    bound_var_fundefs_ctx fdc <--> bound_var_fundefs_ctx (rename_all_fun_ctx_ns sigma fdc)).
+             Proof.
+               intro sig.
+               assert (Hcc := bound_var_rename_all_ns).
+               specialize (Hcc sig).
+               destruct Hcc.               
+               exp_fundefs_ctx_induction IHc IHfdc; intros; simpl; repeat (first [normalize_bound_var_ctx|normalize_bound_var]); split; try (rewrite IHc); try (rewrite IHfdc); try (rewrite <- H); try (rewrite <- H0); auto with Ensembles_DB.
+               rewrite H.
+               simpl.
+               rewrite H with (e := (Ecase v l0)).
+               simpl.
+               eauto with Ensembles_DB.
+               rewrite H with (e:= (Ecase v l)).
+               simpl.
+               rewrite H with (e := (Ecase v l0)).
+               simpl.
+               eauto with Ensembles_DB.
+             Qed.
+
+          Theorem cmap_view_bound_in_ctx:
+            forall sub c v s,
+              cmap_view_ctx sub c ->
+              M.get v sub = Some s ->
+              bound_var_ctx c v.
+          Proof.
+            intros. destruct s; apply H in H0; destructAll.
+            - apply bound_var_ctx_comp_ctx.
+              right; auto.
+            - apply bound_var_ctx_comp_ctx.
+              right.
+              constructor.
+              eapply fundefs_append_bound_vars.
+              reflexivity.
+              right; auto.
+          Qed.
+       
+       
+
+       
+
+    Theorem precontractfun_corresp:
+      forall fds_c fds e c im sub count sig,
+      let ce := (app_ctx_f (rename_all_ctx_ns sig (inlined_ctx_f c im)) (rename_all_ns sig (Efun (fundefs_append fds fds_c) e))) in
+      unique_bindings ce ->
+      closed ce ->
+      c_count ce count ->
+      cmap_view_ctx sub c ->
+      inl_inv im sub ce ->
+      sig_inv_dom sig ce ->
+      forall fds_c' count' sub',
+      precontractfun sig count sub fds_c = (fds_c', count', sub') ->
+      let ce' := (app_ctx_f (rename_all_ctx_ns sig (inlined_ctx_f c im)) (rename_all_ns sig (Efun (fundefs_append fds fds_c') e))) in
+      gsr_clos ce ce' /\ c_count ce' count' /\ inl_inv im sub' ce' /\
+      cmap_view_ctx sub' (comp_ctx_f c (Efun1_c fds_c' Hole_c)).
+    Proof.
+      induction fds_c; intros.
+      - simpl in H5.
+        destruct (get_c v count) eqn:gvc.
+        +  assert (H1v := H1 v).
+           rewrite gvc in H1v.
+           assert (gsr_clos ce
+                             (rename_all_ctx_ns sig (inlined_ctx_f c im)
+                             |[ rename_all_ns sig
+                                           (Efun (fundefs_append fds fds_c) e0) ]|)).
+           { constructor.
+             constructor.             
+             simpl.
+             rewrite rename_all_ns_fundefs_append.
+             rewrite rename_all_ns_fundefs_append.
+             simpl.
+             apply Fun_rem_s.
+             specialize (H1 v).
+             rewrite gvc in H1.
+             unfold ce in H1.
+             apply num_occur_app_ctx in H1. destructAll; pi0.
+             simpl in H6.
+             rewrite rename_all_ns_fundefs_append in H6.
+             simpl in H6. auto.
+           }             
+           assert (Hub' := gsr_preserves_clos _ _ H H0 H6).
+           destruct Hub'.
+           assert (Hse := gsr_preserves_sig_dom _ _ _ H H0 H6 H4).           
+           eapply IHfds_c with (fds := fds) (e := e0) (c := c) (im := im) in H5; eauto.
+           destructAll.
+           unfold ce'.
+           split.
+           eapply rt_trans.
+           apply H6.
+           auto.
+           split; auto.
+           {
+             intro.
+             specialize (H1 v0).
+             unfold ce in H1.
+             apply num_occur_app_ctx in H1.
+             destructAll.
+             simpl in H9. inv H9.
+             rewrite rename_all_ns_fundefs_append in H16.
+             apply fundefs_append_num_occur' in H16.
+             destructAll.
+             simpl in H11.
+             inv H11.
+             eapply num_occur_n.
+             apply num_occur_app_ctx.
+             exists x, (n+(x0 + m)).
+             split; auto.
+             split.
+             simpl.
+             constructor; auto.
+             rewrite rename_all_ns_fundefs_append.
+             eapply fundefs_append_num_occur.
+             reflexivity.
+             auto. auto.
+             reflexivity.
+             symmetry.
+             unfold dec_census.
+             assert  (Hcc := combine_minus_census_correct).
+             destruct Hcc.
+             specialize (H11 e count sig). rewrite <- H11.
+             rewrite gccombine_sub.
+             rewrite H10.
+             assert (c_count (rename_all sig e) (init_census (rename_all sig e))).
+             apply init_census_correct.
+             rewrite (proj1 (rename_all_no_shadow _)) in H14 at 1.
+             specialize (H14 v0).
+             assert (n0 =  get_c v0 (init_census (rename_all sig e))).
+             eapply (proj1 (num_occur_det v0)); eauto.             
+             omega.
+             intro.
+             intros.
+             apply H4 in H15.
+             unfold ce in H15.
+             intro; apply H15.
+             apply bound_var_app_ctx.
+             right.
+             apply bound_var_rename_all_ns.
+             normalize_bound_var.
+             left.
+             rewrite fundefs_append_bound_vars.
+             2: reflexivity.
+             normalize_bound_var.
+             auto.
+           }
+           {
+             intro.
+             intros.
+             apply H3 in H9.
+             destruct H9.
+             split; [| split].
+             - intro.
+               apply H9.
+               unfold ce.
+               apply bound_var_app_ctx in H11.
+               apply bound_var_app_ctx.
+               inv H11; auto.
+               right.
+               apply bound_var_rename_all_ns.
+               apply bound_var_rename_all_ns in H12.
+               normalize_bound_var.
+               rewrite bound_var_Efun in H12.
+               inv H12; auto.
+               left.
+               rewrite fundefs_append_bound_vars.
+               2: reflexivity.
+               rewrite fundefs_append_bound_vars in H11.
+               2: reflexivity.
+               rewrite bound_var_fundefs_Fcons.
+               inv H11; auto.
+             - apply H10 in H11.
+               unfold ce in H11.
+               intro. intro.
+               inv H11.
+               specialize (H13 x).
+               apply H13.
+               inv H12. split; auto.
+               rewrite bound_var_app_ctx in H11.
+               rewrite bound_var_app_ctx.
+               inv H11; auto.
+               right.
+               apply bound_var_rename_all_ns.
+               apply bound_var_rename_all_ns in H12.
+               normalize_bound_var.
+               rewrite bound_var_Efun in H12.
+               inv H12; auto.
+               left.
+               rewrite fundefs_append_bound_vars.
+               2: reflexivity.
+               rewrite fundefs_append_bound_vars in H11.
+               2: reflexivity.
+               rewrite bound_var_fundefs_Fcons.
+               inv H11; auto.               
+           }
+          
+        +           assert (rename_all_ctx_ns sig (inlined_ctx_f c im)
+        |[ rename_all_ns sig
+                      (Efun (fundefs_append fds (Fcons v f l e fds_c)) e0) ]| =
+                                                                              rename_all_ctx_ns sig (inlined_ctx_f c im)
+        |[ rename_all_ns sig
+                      (Efun (fundefs_append (fundefs_append fds (Fcons v f l e Fnil)) fds_c) e0) ]|) by 
+              (rewrite <- fundefs_append_assoc; reflexivity).
+          unfold ce in IHfds_c.
+          fold ce in H6. rewrite H6 in *.
+          destruct  (precontractfun sig count sub fds_c ) eqn:prefun.
+          destruct p.
+          specialize (IHfds_c  _ _ _ _ _ _ _ H H0 H1 H2 H3 H4 _ _ _ prefun).
+          inv H5.
+          assert (rename_all_ctx_ns sig (inlined_ctx_f c im)
+         |[ rename_all_ns sig (Efun (fundefs_append fds (Fcons v f l e f0)) e0)
+          ]| =
+             rename_all_ctx_ns sig (inlined_ctx_f c im)
+         |[ rename_all_ns sig (Efun (fundefs_append (fundefs_append fds (Fcons v f l e Fnil))  f0) e0)
+          ]|).
+          rewrite <-fundefs_append_assoc; reflexivity.          
+          unfold ce'.
+          rewrite H5.
+          destructAll.
+          split; auto.
+          split; auto.
+          split; auto.
+          clear H10.
+          intro. intro. apply H9 in H10.          
+          destruct H10.
+          split; auto.
+          intros.
+          destruct (var_dec f1 v).
+                    * subst.
+                      exfalso.
+                      apply H10.
+                      apply bound_var_app_ctx.
+                      right.
+                      rewrite <- (proj1 (bound_var_rename_all_ns _)).
+                      rewrite bound_var_Efun.
+                      left.
+                      rewrite fundefs_append_bound_vars.
+                      2: reflexivity.
+                      left.
+                      rewrite fundefs_append_bound_vars.
+                      2: reflexivity.
+                      right.
+                      rewrite bound_var_fundefs_Fcons.
+                      left; auto.
+                    * rewrite M.gso in H12.
+                      apply H11 in H12.
+                      auto. auto.
+                    * apply cmap_view_efun1_cons. apply H10.
+                      
+                      (* due to unique binding *)
+
+                      apply (gsr_preserves_clos _ _ H H0) in H7.
+                      destruct H7.
+                      destruct (M.get v c0) eqn:gvc0.
+                      2: auto.
+
+                      assert (bound_var_ctx (comp_ctx_f c (Efun1_c f0 Hole_c)) v).
+                      eapply cmap_view_bound_in_ctx; eauto.                      
+
+                      apply bound_var_ctx_comp_ctx in H12.
+                      apply ub_app_ctx_f in H7.
+                      destructAll.
+                      exfalso.
+                      inv H12.
+                      {
+                        inv H14.
+                        specialize (H12 v).
+                        apply H12.
+                        split.
+                        apply bound_var_ctx_rename_all_ns.
+                        {
+                          destruct s.
+                          - apply H10 in gvc0. destructAll.
+                            apply comp_ctx_split in H14.
+                            destruct H14.
+                            + destructAll.
+                              destruct x1; inv H14.
+                              rewrite (proj1 inlined_comp_ctx).
+                              simpl.                            
+                              apply bound_var_ctx_comp_ctx.
+                              right; auto.
+                            + destructAll. destruct x2; inv H17. destruct x2; inv H18.
+                          - assert (gvc0' := gvc0).
+                            apply H10 in gvc0. destructAll.
+                            apply comp_ctx_split in H14.
+                            destruct H14.
+                            + destructAll.
+                              destruct x3; inv H14.
+                              * simpl in H13.
+                                inv H13.
+                                repeat rewrite rename_all_ns_fundefs_append in H18.
+                                eapply fundefs_append_unique_bindings_l in H18.
+                                2: reflexivity.
+                                destructAll.
+                                inv H16.
+                                exfalso. specialize (H18 v).
+                                apply H18.                                
+                                split.
+                                eapply fundefs_append_bound_vars.
+                                reflexivity. right.
+                                simpl. auto.
+                                eapply fundefs_append_bound_vars.
+                                reflexivity. right.
+                                simpl. auto.                              
+                              * rewrite (proj1 inlined_comp_ctx).
+                                apply bound_var_ctx_comp_ctx. right. simpl.
+                                rewrite inlined_fundefs_append.
+                                simpl. destruct (get_b v im) eqn:gbvim.
+                                apply H3 in gbvim. destructAll.
+                                exfalso.
+                                apply H14.
+                                apply bound_var_app_ctx.
+                                right.
+                                apply bound_var_rename_all_ns.
+                                constructor.
+                                eapply fundefs_append_bound_vars.
+                                reflexivity.
+                                left.
+                                eapply fundefs_append_bound_vars.
+                                reflexivity.  
+                                right.
+                                auto.
+                                constructor.
+                                eapply fundefs_append_bound_vars.
+                                reflexivity.  
+                                right.
+                                auto.
+                            + destructAll.
+                              destruct x4; inv H17.
+                              * exfalso.
+                                simpl in H13.
+                                inv H13.
+                                repeat rewrite rename_all_ns_fundefs_append in H18.
+                                eapply fundefs_append_unique_bindings_l in H18.
+                                2: reflexivity.
+                                destructAll.
+                                inv H16.
+                                exfalso. specialize (H18 v).
+                                apply H18.                                
+                                split.
+                                eapply fundefs_append_bound_vars.
+                                reflexivity. right.
+                                simpl. auto.
+                                eapply fundefs_append_bound_vars.
+                                reflexivity. right.
+                                simpl. auto.                              
+                              * destruct x4; inv H18.
+                        }
+                        apply bound_var_rename_all_ns.
+                        constructor.
+                        eapply fundefs_append_bound_vars.
+                        reflexivity.
+                        left.
+                        eapply fundefs_append_bound_vars.
+                        reflexivity.
+                        right.
+                        auto.                        
+                      }
+                      {
+                        simpl in H13. inv H13.
+                        rewrite rename_all_ns_fundefs_append in H18.
+                        rewrite rename_all_ns_fundefs_append in H18.
+                        eapply fundefs_append_unique_bindings_l in H18.
+                        2: reflexivity.
+                        destructAll.
+                        inv H16. specialize (H18 v).
+                        apply H18.
+                        split.
+                        eapply fundefs_append_bound_vars.
+                        reflexivity.
+                        right. simpl. auto.
+                        apply bound_var_rename_all_ns.
+                        inv H15. 
+                        auto.
+                        inv H22.
+                      }
+      - simpl in H5. inv H5.
+        split.
+        apply rt_refl.
+        split; auto.
+        split; auto.
+        apply cmap_view_efun1_nil. auto.
+    Qed.
+
+
+    Theorem bound_var_fundefs_inlined:
+  forall im1 im2,
+    b_map_le im1 im2 ->
+    forall fds,
+    Included _ (bound_var_fundefs (inlined_fundefs_f fds im2)) (bound_var_fundefs (inlined_fundefs_f fds im1)).
+    Proof.
+      intros im1 im2 Him; induction fds; simpl; repeat normalize_bound_var; auto.
+      - destruct (get_b v im1) eqn:gbvi.
+        + apply Him in gbvi. rewrite gbvi. auto.
+        + destruct (get_b v im2); repeat normalize_bound_var; eauto with Ensembles_DB.
+      - intro. intro. inv H.
+    Qed.
+        
+    Lemma bound_var_ctx_inlined_antimon_mut:
+      forall im1 im2,
+        b_map_le im1 im2 ->
+        (forall c, 
+           Included _ (bound_var_ctx (inlined_ctx_f c im2)) (bound_var_ctx (inlined_ctx_f c im1))) /\
+        (forall fdc, 
+           Included _ (bound_var_fundefs_ctx (inlined_fundefs_ctx_f fdc im2)) (bound_var_fundefs_ctx (inlined_fundefs_ctx_f fdc im1))).
+    Proof.
+      intros im1 im2 Him.
+      exp_fundefs_ctx_induction IHc1 IHfc1; simpl; repeat normalize_bound_var_ctx; eauto with Ensembles_DB.
+      - intro.
+        repeat normalize_bound_var_ctx.
+        eauto with Ensembles_DB.
+      - apply Included_Union_compat; auto.
+        apply bound_var_fundefs_inlined; auto.
+    Qed.
+
+    Theorem bound_var_ctx_inlined_antimon:
+      forall im1 im2 c,
+        b_map_le im1 im2 ->
+           Included _ (bound_var_ctx (inlined_ctx_f c im2)) (bound_var_ctx (inlined_ctx_f c im1)). 
+    Proof.
+      intros.
+      apply bound_var_ctx_inlined_antimon_mut; auto.
+    Qed.
+
+
+        Theorem bound_var_fundefs_ctx_inlined_antimon:
+      forall im1 im2 fdc,
+        b_map_le im1 im2 ->
+          Included _ (bound_var_fundefs_ctx (inlined_fundefs_ctx_f fdc im2)) (bound_var_fundefs_ctx (inlined_fundefs_ctx_f fdc im1)).
+    Proof.
+      intros.
+      apply bound_var_ctx_inlined_antimon_mut; auto.
+    Qed.
+
+    
+    (* used for function and constructor case *)
+    Theorem sub_none_from_pre:
+      forall c im e v sub sig,
+        unique_bindings (rename_all_ctx_ns sig (inlined_ctx_f c im) |[ e ]|) ->
+      cmap_view_ctx sub c ->
+      inl_inv im sub (rename_all_ctx_ns sig (inlined_ctx_f c im) |[ e ]|) ->
+      bound_var e v ->
+      M.get v sub = None.
+    Proof.
+      intros.
+      destruct (M.get v sub) eqn:gvs; auto.
+      exfalso.
+      destruct s; apply H0 in gvs; destructAll.
+      - apply ub_app_ctx_f in H.
+        destructAll.
+        inv H4.
+        specialize (H5 v).
+        apply H5.
+        split.
+        apply bound_var_ctx_rename_all_ns.
+        rewrite (proj1 inlined_comp_ctx).
+        apply bound_var_ctx_comp_ctx.
+        right.
+        simpl. auto.
+        auto.
+      - apply ub_app_ctx_f in H.
+        destructAll.
+        inv H4.
+        specialize (H5 v).
+        apply H5.
+        split.
+        apply bound_var_ctx_rename_all_ns.
+        rewrite (proj1 inlined_comp_ctx).
+        apply bound_var_ctx_comp_ctx.
+        right.
+        simpl.
+        constructor.
+        rewrite inlined_fundefs_append.
+        simpl. destruct (get_b v im) eqn:gbvi.
+        + apply H1 in gbvi.
+          exfalso.
+          destruct gbvi. apply H4.
+          apply bound_var_app_ctx.
+          right. auto.
+        + eapply fundefs_append_bound_vars.
+          reflexivity.
+          right. simpl; auto.
+        + auto.
+    Qed.
+
+    Ltac ctx_inl_push :=
+        rewrite (proj1 inlined_comp_ctx);
+        simpl;
+        rewrite (proj1 (rename_all_ctx_ns_comp_ctx _ _));
+        symmetry;
+        rewrite <- app_ctx_f_fuse;
+        simpl; auto.
+
+
+    
+    Theorem nthN_map:
+      forall A B  f l n v,
+      nthN l n = Some v ->
+      nthN (@map A B f l) n = Some (f v).
+    Proof.
+      induction l; intros.
+      - inv H.
+      - simpl in H. destruct n.
+        simpl. inv H; auto.
+        apply IHl.
+        simpl. destruct p. apply H.
+        apply H.
+        apply H.
+    Qed.        
+
+   
+                   (* will need to prove at the same time postcontractfun and contractcase *)
+    Theorem shrink_corresp:
+      forall e sub im sig c count,
+      let ce := (app_ctx_f (rename_all_ctx_ns sig (inlined_ctx_f c im)) (rename_all_ns sig e)) in
+      unique_bindings ce ->
+      closed ce ->
+      c_count ce count ->
+      cmap_view_ctx sub c ->
+      inl_inv im sub ce ->
+      sig_inv_dom sig ce ->
+      forall e' count' im' BP,
+        contract sig count e sub im = existT _ (e', count', im') BP ->
+        let ce' := (app_ctx_f (rename_all_ctx_ns sig (inlined_ctx_f c im')) e') in
+      gsr_clos ce ce' /\ c_count ce' count' /\ inl_inv im' sub ce'.
+    Proof.
+      intros e sub inl. remember (1 + term_sub_inl_size (e, sub,inl)) as n. assert (n > term_sub_inl_size (e, sub, inl)). omega. clear Heqn. revert e sub inl H. induction n; intros. inversion H. destruct e; rewrite contract_eq in H6.
+      - (* constr *)
+        destruct (get_c v count) eqn:gvc.
+        + (* dead constr *)
+          simpl in ce.
+          assert (gsr_clos ce (rename_all_ctx_ns sig (inlined_ctx_f c inl) |[ (rename_all_ns sig e) ]|)).
+          { unfold ce.
+            constructor. constructor.
+            constructor.
+            specialize (H2 v). unfold ce in H2.
+            apply num_occur_app_ctx in H2. rewrite gvc in H2. destructAll; pi0.
+            inv H7; pi0; auto. rewrite H8. auto.
+          }
+          assert (Hub := gsr_preserves_clos _ _ H0 H1 H7).
+          destruct Hub as (Hub, Hdj).
+          assert (Hse := gsr_preserves_sig_dom _ _ _ H0 H1 H7 H5).           
+          simpl in H6.
+          eapply IHn in H6; eauto.
+          destruct H6.
+          destruct H8.
+          unfold ce'.
+          split.
+          eapply rt_trans.
+          apply H7.
+          auto.
+          split; auto.
+          unfold term_sub_inl_size in *. simpl in *.
+          omega.
+          {
+            intro. specialize (H2 v0).
+            unfold ce in H2.
+            apply num_occur_app_ctx in H2. destructAll.
+            inv H8.
+            apply num_occur_app_ctx.
+            exists x, n0.
+            repeat split; auto.
+            unfold dec_census_list.
+            rewrite <- combine_minus_census_list.
+            rewrite gccombine_sub.
+            rewrite H9.
+            rewrite update_census_list_correct.
+            rewrite apply_r_list_empty.
+            unfold get_c. rewrite M.gempty. omega.
+          }
+          intro. intros. apply H4 in H8.
+          destructAll.
+          assert (Included _ (bound_var (rename_all_ctx_ns sig (inlined_ctx_f c inl) |[ rename_all_ns sig e ]|)) (bound_var ce)).
+          unfold ce.
+          repeat rewrite bound_var_app_ctx.
+          apply Included_Union_compat.
+          reflexivity.
+          rewrite bound_var_Econstr. left; auto.          
+          split; auto.
+          intro; apply H8.
+          apply H10. auto.
+          intros. apply H9 in H11.
+          eapply Disjoint_Included_l.
+          2: apply H11. auto.          
+        + (* live constr *)
+          assert (M.get v sub = None) by (eapply sub_none_from_pre; simpl; eauto; simpl; auto).
+          
+          assert (rename_all_ctx_ns sig (inlined_ctx_f c inl)
+                 |[ rename_all_ns sig (Econstr v c0 l e)]|  =
+                 (rename_all_ctx_ns sig (inlined_ctx_f (comp_ctx_f c (Econstr_c v c0 l Hole_c)) inl)
+                 |[ rename_all_ns sig e ]|)) by ctx_inl_push.
+          remember (contract sig count e (M.set v (SVconstr c0 l) sub) inl).
+          symmetry in Heqs.
+          destruct s.
+          destruct x.
+          destruct p.
+          eapply IHn with (c := (comp_ctx_f c (Econstr_c v c0 l Hole_c))) in Heqs; unfold ce in *; try rewrite H8 in *; eauto.
+          {
+            destruct Heqs. destruct H10.
+             assert (rename_all_ctx_ns sig (inlined_ctx_f c im')
+                     |[ Econstr v c0 (apply_r_list sig l) e0 ]| = 
+               (rename_all_ctx_ns sig
+            (inlined_ctx_f (comp_ctx_f c (Econstr_c v c0 l Hole_c)) im')
+               |[ e0 ]|)).              
+              rewrite (proj1 inlined_comp_ctx).
+              rewrite (proj1 (rename_all_ctx_ns_comp_ctx _ _)).              
+            rewrite <- app_ctx_f_fuse.
+            simpl. auto.            
+            
+            destruct (get_c v c1) eqn:gvc1.
+            - (* dead post *)
+              inv H6.
+              split.
+              2: split.
+              + eapply rt_trans.
+                apply H9.
+                rewrite <- H12.
+                unfold ce'.
+                constructor.
+                constructor.
+                constructor.
+                specialize (H10 v).
+                rewrite gvc1 in H10.
+                apply num_occur_app_ctx in H10; destructAll; pi0; auto.
+              + intro. specialize (H10 v0).
+                unfold ce'.
+                apply num_occur_app_ctx in H10. destructAll.
+                rewrite (proj1 inlined_comp_ctx) in H6.
+                rewrite (proj1 (rename_all_ctx_ns_comp_ctx _ _)) in H6.
+                
+                apply num_occur_ec_comp_ctx in H6; destructAll.
+                simpl in H14. inv H14. inv H21. simpl in H13.                                
+                
+                apply num_occur_app_ctx.
+                exists x1, x0. split; auto. split; auto.
+                
+                unfold dec_census_list.
+                rewrite <- combine_minus_census_list.
+                rewrite gccombine_sub.
+                rewrite H13.
+                rewrite update_census_list_correct.
+                rewrite apply_r_list_empty.
+                unfold get_c. rewrite M.gempty. omega.
+              + split; intros.
+                assert (H6' := H6).
+                apply H11 in H6.                
+                destruct H6.
+                intro; apply H6.
+                unfold ce' in H14.              
+                apply bound_var_app_ctx in H14.
+                apply bound_var_app_ctx. inv H14.
+                left. rewrite (proj1 inlined_comp_ctx).
+                rewrite (proj1 (rename_all_ctx_ns_comp_ctx _ _)).
+                rewrite (proj1 bound_var_ctx_comp_ctx).
+                left; auto. right; auto.                 
+                apply H11 in H6. destruct H6.
+                destruct (var_dec f v).
+                * exfalso.
+                  apply H6; subst.
+                  apply bound_var_app_ctx.
+                  left. rewrite (proj1 inlined_comp_ctx).
+                  rewrite (proj1 (rename_all_ctx_ns_comp_ctx _ _)).
+                  rewrite (proj1 bound_var_ctx_comp_ctx).
+                  right.
+                  simpl. auto.
+                *
+                  assert ( M.get f (M.set v (SVconstr c0 l) sub) = Some (SVfun t xs m) ).
+                  rewrite M.gso; auto. 
+                  apply H14 in H15. 
+                  eapply Disjoint_Included_l.
+                  2: apply H15.
+                  unfold ce'.
+                  do 2 (rewrite bound_var_app_ctx).
+                  rewrite (proj1 inlined_comp_ctx).
+                  rewrite (proj1 (rename_all_ctx_ns_comp_ctx _ _)).
+                  rewrite (proj1 bound_var_ctx_comp_ctx).
+                  eauto with Ensembles_DB.
+            - (* live post *)
+              inv H6.
+              unfold ce'; rewrite H12.
+              split; auto.
+              split; auto.
+              intro. intros.
+              assert (H6' := H6).
+              apply H11 in H6. destruct H6.
+              split; auto.
+              intros.
+              destruct (var_dec f v).
+              + (* impossible, then v is inlined but bound *)
+                exfalso.
+                subst.
+                apply H11 in H6'.
+                destruct H6'.
+                apply H15.
+                rewrite (proj1 inlined_comp_ctx).
+                rewrite (proj1 (rename_all_ctx_ns_comp_ctx _ _)).
+                apply bound_var_app_ctx.
+                left.
+                apply bound_var_ctx_comp_ctx.
+                right. simpl. constructor.
+              + assert ( M.get f (M.set v (SVconstr c0 l) sub) = Some (SVfun t xs m)).
+                rewrite M.gso; auto.
+                apply H13 in H15. auto.              
+          }          
+          (* size *)
+          eapply NPeano.Nat.lt_le_trans.
+          apply constr_sub_size.
+          omega.
+          (* cmap_view *)
+          apply cmap_view_constr; eauto.
+          (* inl_inv *)
+          { intro. intros. apply H4 in H9.
+            destruct H9.
+            split; auto.
+            intros.
+            destruct (var_dec f v).
+            subst.
+            rewrite M.gss in H11. inv H11.
+            rewrite M.gso in H11; auto.
+            eapply H10; eauto.
+          }
+      - (* case *)
+        simpl in H6. 
+        destruct ( M.get (apply_r sig v) sub ) eqn:garvs; [destruct s|].
+        +  destruct (findtag l c0) eqn:ftlc0.
+           * (* folded case *)
+             
+             admit.
+           * (* case not found, same as fun *)
+             admit.
+        + (* fun *)
+          admit.
+        + (* None *)
+          admit.
+      - (* proj *)
+        simpl in H6.
+        destruct (M.get (apply_r sig v0) sub) eqn:garv0s; [destruct s|].
+        + (* constr *)
+          destruct (nthN l n0) eqn:n0thl.
+          * (* constant folding *)
+            assert (Hgvs : M.get v sig = None).
+            { destruct (M.get v sig) eqn:gvs.
+              apply H5 in gvs. exfalso.
+              apply gvs.
+              apply bound_var_app_ctx.
+              right; simpl; auto.
+              auto.
+            }
+            assert (Hbv :
+                      ~ bound_var_ctx
+                      (rename_all_ctx_ns sig (inlined_ctx_f c inl)) v).
+            {
+              unfold ce in H0. apply ub_app_ctx_f in H0.
+              intro.
+              destructAll.
+              inv H9.
+              specialize (H10 v).
+              apply H10.
+              split; simpl; auto.
+            }
+            apply H3 in garv0s.
+            destructAll.
+            assert (gsr_clos (rename_all_ctx_ns sig
+                                                (inlined_ctx_f (comp_ctx_f x (Econstr_c (apply_r sig v0) c1 l x0))
+                                                               inl) |[ rename_all_ns sig (Eproj v c0 n0 v0 e) ]|)
+                             (rename_all_ctx_ns (M.set v (apply_r sig v1) sig)
+                                                (inlined_ctx_f (comp_ctx_f x (Econstr_c (apply_r sig v0) c1 l x0)) inl)
+                             |[ rename_all_ns (M.set v (apply_r sig v1) sig) e ]|)).
+            { eapply rt_trans.
+              - simpl.
+                rewrite (proj1 inlined_comp_ctx).
+                simpl.
+                rewrite (proj1 (rename_all_ctx_ns_comp_ctx _ _)).
+                rewrite <- app_ctx_f_fuse.
+                simpl. constructor.
+                constructor. apply Constr_proj_s.
+                unfold apply_r_list.
+                apply nthN_map. eauto.
+              - (* 2 parts : *)
+                destruct (M.get v sig) eqn:gvs.
+                inv Hgvs.
+                (*) context is unchanged by extra sig *)
+                assert (
+                     (rename_all_ctx_ns (M.set v (apply_r sig v1) sig)
+                                        (inlined_ctx_f (comp_ctx_f x (Econstr_c (apply_r sig v0) c1 l x0)) inl) =
+                      (rename_all_ctx_ns sig
+                                         (inlined_ctx_f (comp_ctx_f x (Econstr_c (apply_r sig v0) c1 l x0)) inl)))).
+                {
+                  apply eq_P_rename_all_ctx_ns.
+                  intro; intro.
+                  destruct (var_dec x1 v).
+                  - subst. exfalso.
+                    apply H7.
+                    eapply not_occur_rename_ctx_not_dom with (sig := sig).
+                    intro. inv H8. rewrite gvs in H9; inv H9.
+                    assert (~ occurs_free_ctx (rename_all_ctx_ns sig
+            (inlined_ctx_f
+               (comp_ctx_f x (Econstr_c (apply_r sig v0) c1 l x0)) inl)) v).
+                    intro.
+                    apply closed_app_ctx in H1.
+                    apply H1 in H8. inv H8.
+                    apply not_free_dead_or_bound_ctx in H8.
+                    inv H8; auto.
+                    exfalso; auto.                                        
+                  - rewrite M.gso; auto.
+                }                    
+                rewrite H7.
+                admit.
+                
+                (* 1) rename v (rename_all e) = rename_all+v e by  *)
+                
+                
+
+                
+            }                
+            assert (Hub' := gsr_preserves_clos _ _ H0 H1 H7).
+            destructAll.
+            assert (Hse := gsr_preserves_sig_dom _ _ _ H0 H1 H7 H5).
+            eapply IHn in H6; eauto.
+            assert (rename_all_ctx_ns (M.set v (apply_r sig v1) sig)
+            (inlined_ctx_f
+               (comp_ctx_f x (Econstr_c (apply_r sig v0) c1 l x0)) im')  =
+                     (rename_all_ctx_ns sig 
+            (inlined_ctx_f
+               (comp_ctx_f x (Econstr_c (apply_r sig v0) c1 l x0)) im'))).
+            {
+              apply eq_P_rename_all_ctx_ns.
+              intro; intro.
+              destruct (var_dec x1 v).
+              - subst.
+                exfalso.
+                apply H10.
+                admit.
+                SearchAbout b_map_le bound_var.
+              - rewrite M.gso by auto; auto.
+            }
+            rewrite H10 in *.
+            destructAll.
+            split; auto.
+            eapply rt_trans.
+            2: apply H6.
+            apply H7.
+            {             (* size *)
+              unfold term_sub_inl_size in *.
+              simpl in *; omega.
+            }
+            {             (* c_count *)
+              admit.
+            }
+            {            (* inl_inv *)
+              intro. intros.
+              apply H4 in H10. unfold ce in H10.
+              destruct H10.
+              split.
+              - intro; apply H10.
+                apply bound_var_app_ctx in H12.
+                inv H12.
+                rewrite <- (proj1 (bound_var_ctx_rename_all_ns _ )) in H13.
+                apply bound_var_app_ctx.
+                left.
+                rewrite <- (proj1 (bound_var_ctx_rename_all_ns _ )).
+                auto.
+                apply bound_var_app_ctx.
+                right.
+                apply bound_var_rename_all_ns.
+                apply bound_var_rename_all_ns in H13.                
+                auto.
+              - intros. apply H11 in H12.
+                eapply Disjoint_Included_l.
+                2: apply H12.
+                do 2 rewrite bound_var_app_ctx.
+                
+                do 2 (rewrite <- (proj1 (bound_var_ctx_rename_all_ns _ ))).
+                do 2 (rewrite <- (proj1 (bound_var_rename_all_ns _ ))).
+                normalize_bound_var.
+                auto with Ensembles_DB.
+            }
+            {            (* sig_inv *)
+              intro. intros.
+              destruct (var_dec x1 v).
+              - subst. rewrite M.gss in H10.
+                inv H10.
+                intro.
+                unfold ce in H0.
+                apply ub_app_ctx_f in H0.
+                destructAll.
+                apply bound_var_app_ctx in H10.
+                inv H10.
+                apply bound_var_ctx_rename_all_ns in H13.
+                inv H12.
+                specialize (H10 v).
+                apply H10.
+                split.
+                2: simpl; auto.
+                apply bound_var_ctx_rename_all_ns.
+                auto.
+                apply bound_var_rename_all_ns in H13.
+                simpl in H11. inv H11.
+                apply H15.
+                apply bound_var_rename_all_ns. auto.
+              - rewrite M.gso in H10 by auto.
+                apply Hse in H10.
+                auto.
+            }
+          * (* same as fun and none *)
+            assert (rename_all_ctx_ns sig (inlined_ctx_f c inl)
+                   |[ rename_all_ns sig (Eproj v c0 n0 v0 e) ]| =
+                    rename_all_ctx_ns sig (inlined_ctx_f (comp_ctx_f c (Eproj_c v c0 n0 v0 Hole_c)) inl)
+                   |[ rename_all_ns sig e ]|) by             ctx_inl_push.
+            remember (contract sig count e sub inl).
+            destruct s. destruct x. destruct p.
+            symmetry in Heqs.
+            unfold ce in *; rewrite H7 in *.
+            eapply IHn in Heqs; eauto.
+            destructAll.
+            inv H6.
+            assert ( (rename_all_ctx_ns sig
+            (inlined_ctx_f (comp_ctx_f c (Eproj_c v c0 n0 v0 Hole_c)) im')
+                     |[ e0 ]|) = rename_all_ctx_ns sig (inlined_ctx_f c im')
+                    |[ Eproj v c0 n0 (apply_r sig v0) e0 ]|) by  ctx_inl_push. 
+            unfold ce';  rewrite <- H6.
+            split; auto.
+            unfold term_sub_inl_size in *. simpl. simpl in H. omega.
+            apply cmap_view_proj; auto.
+        + (* fun *)
+         assert (rename_all_ctx_ns sig (inlined_ctx_f c inl)
+                   |[ rename_all_ns sig (Eproj v c0 n0 v0 e) ]| =
+                    rename_all_ctx_ns sig (inlined_ctx_f (comp_ctx_f c (Eproj_c v c0 n0 v0 Hole_c)) inl)
+                   |[ rename_all_ns sig e ]|) by             ctx_inl_push.
+            remember (contract sig count e sub inl).
+            destruct s. destruct x. destruct p.
+            symmetry in Heqs.
+            unfold ce in *; rewrite H7 in *.
+            eapply IHn in Heqs; eauto.
+            destructAll.
+            inv H6.
+            assert ( (rename_all_ctx_ns sig
+            (inlined_ctx_f (comp_ctx_f c (Eproj_c v c0 n0 v0 Hole_c)) im')
+                     |[ e1 ]|) = rename_all_ctx_ns sig (inlined_ctx_f c im')
+                    |[ Eproj v c0 n0 (apply_r sig v0) e1 ]|) by  ctx_inl_push. 
+            unfold ce';  rewrite <- H6.
+            split; auto.
+            unfold term_sub_inl_size in *. simpl. simpl in H. omega.
+            apply cmap_view_proj; auto. 
+        + (* none *)
+         assert (rename_all_ctx_ns sig (inlined_ctx_f c inl)
+                   |[ rename_all_ns sig (Eproj v c0 n0 v0 e) ]| =
+                    rename_all_ctx_ns sig (inlined_ctx_f (comp_ctx_f c (Eproj_c v c0 n0 v0 Hole_c)) inl)
+                   |[ rename_all_ns sig e ]|) by             ctx_inl_push.
+            remember (contract sig count e sub inl).
+            destruct s. destruct x. destruct p.
+            symmetry in Heqs.
+            unfold ce in *; rewrite H7 in *.
+            eapply IHn in Heqs; eauto.
+            destructAll.
+            inv H6.
+            assert ( (rename_all_ctx_ns sig
+            (inlined_ctx_f (comp_ctx_f c (Eproj_c v c0 n0 v0 Hole_c)) im')
+                     |[ e0 ]|) = rename_all_ctx_ns sig (inlined_ctx_f c im')
+                    |[ Eproj v c0 n0 (apply_r sig v0) e0 ]|) by  ctx_inl_push. 
+            unfold ce';  rewrite <- H6.
+            split; auto.
+            unfold term_sub_inl_size in *. simpl. simpl in H. omega.
+            apply cmap_view_proj; auto. 
+      - (* fun *)
+        remember (precontractfun sig count sub f).
+        destruct p.
+        destruct p.
+        symmetry in Heqp.
+        assert (Heqp' := Heqp).
+        eapply precontractfun_corresp with (fds := Fnil) in Heqp; eauto.
+        destructAll.
+        assert (Hub' := gsr_preserves_clos _ _ H0 H1 H7).
+        destruct Hub'.
+        assert (Hse := gsr_preserves_sig_dom _ _ _ H0 H1 H7 H5).
+        simpl in *.
+        assert ((rename_all_ctx_ns sig (inlined_ctx_f c inl)
+                |[ rename_all_ns sig (Efun f0 e) ]|) =
+                (rename_all_ctx_ns sig (inlined_ctx_f (comp_ctx_f c (Efun1_c f0 Hole_c)) inl)
+                |[ rename_all_ns sig e ]|)).
+        {
+          ctx_inl_push.
+          rewrite Disjoint_inlined_fds.
+          reflexivity.
+          split. intros. intro.
+          destruct H13.
+          inv H14. apply H9 in H16.
+          destruct H16.
+          apply H14.
+          apply bound_var_app_ctx.
+          right.
+          constructor.
+          apply bound_var_rename_all_ns.
+          auto.
+        }
+        simpl in H13.
+        rewrite H13 in *.
+        remember (contract sig c1 e c0 inl ).
+        destruct s. destruct x.
+        destruct p.
+        symmetry in Heqs.
+        eapply IHn in Heqs; eauto.
+        destructAll.
+        (* show that e0 = rename_all_ns sig e0 *)
+        (* replace f0 by fundefs_append Fnil f0 *)
+        (* use postcontractfun_corresp *)
+        admit.
+        {
+          assert ((forall im, sub_inl_size c0 im <= funs_size f + sub_inl_size sub im /\ funs_size f0 <= funs_size f))%nat. eapply precontractfun_size. eauto.  unfold term_sub_inl_size. simpl. unfold term_sub_inl_size in H; simpl in H. specialize (H14 inl). omega.
+        }          
+      - (* app *)
+        simpl in H6.
+        destruct (get_c (apply_r sig v) count) eqn:garvc; [ | destruct n0].
+        
+        + (* dead fun -> impossible*)
+          exfalso.
+          specialize (H2 (apply_r sig v)).
+          rewrite garvc in H2.
+          unfold ce in H2.
+          apply num_occur_app_ctx in H2.
+          destructAll; pi0.
+          simpl in H7. inv H7.
+          destruct (cps_util.var_dec (apply_r sig v) (apply_r sig v)).
+          inv H13.
+          apply n0; auto.
+        + (* only occ *)
+          destruct ( M.get (apply_r sig v) sub ) eqn:garvs; [destruct s|].
+          * (* constr, ill-typed but eh *)
+            inv H6.
+            unfold ce in *; unfold ce' in *.
+            split; auto.
+            simpl. apply rt_refl.                    
+          * (* function inlining *)
+            assert (garvs' := garvs).
+            apply H3 in garvs.
+            destructAll.
+            simpl in ce.
+            assert (rename_all_ctx_ns sig
+                                      (inlined_ctx_f
+                                         (comp_ctx_f x
+                                                     (Efun1_c
+                                                        (fundefs_append x1 (Fcons (apply_r sig v) f0 l0 e x2)) x0))
+                                         inl) |[ Eapp (apply_r sig v) f (apply_r_list sig l) ]| =
+                                                                                                (rename_all_ctx_ns sig (inlined_ctx_f x inl)) |[ 
+                      Efun (fundefs_append (rename_all_fun_ns sig (inlined_fundefs_f x1 inl)) (Fcons (apply_r sig v) f0 l0 (rename_all_ns sig e) (rename_all_fun_ns sig (inlined_fundefs_f x2 inl)))) (rename_all_ctx_ns sig (inlined_ctx_f x0 inl) |[ Eapp (apply_r sig v) f (apply_r_list sig l)  ]|)
+                    ]|).
+            {
+              ctx_inl_push.
+              rewrite inlined_fundefs_append.
+              rewrite rename_all_ns_fundefs_append.
+              simpl.
+              destruct (get_b (apply_r sig v) inl) eqn:gbvi.
+              - (* impossible because not dead *)
+                exfalso.
+                apply H4 in gbvi.
+                destructAll.                
+                apply not_bound_dead_or_free in H7.
+                inv H7.
+                2: apply H1 in H9; inv H9.
+                
+                apply num_occur_app_ctx in H9.
+                destructAll; pi0.
+                inv H9.
+                destruct ( cps_util.var_dec (apply_r sig v) (apply_r sig v)).
+                inv H15.
+                apply n0; auto.
+              - simpl. reflexivity.
+            }
+            admit.
+          * (* not a known function *)
+            inv H6.
+            unfold ce in *; unfold ce' in *.
+            split; auto.
+            simpl. apply rt_refl.                    
+        + (* multiple occ *)
+          inv H6.
+          unfold ce in *; unfold ce' in *.
+          split; auto.
+          simpl. apply rt_refl.                    
+      - (* prim -- TODO: modify contract to check for dead prim post *)
+        simpl in H6.
+        assert ( rename_all_ctx_ns sig (inlined_ctx_f c inl)
+                |[ rename_all_ns sig (Eprim v p l e) ]| =
+                 rename_all_ctx_ns sig (inlined_ctx_f (comp_ctx_f c (Eprim_c v p l Hole_c)) inl) |[ rename_all_ns sig e ]|) by ctx_inl_push.
+        remember (contract sig count e sub inl ).
+        destruct s.        
+        destruct x. destruct p0.
+        symmetry in Heqs.
+        eapply  IHn with (c := (comp_ctx_f c (Eprim_c v p l Hole_c))) in Heqs; try (rewrite <- H7; eauto).
+        3: (apply cmap_view_prim; auto).
+        assert ((rename_all_ctx_ns sig
+              (inlined_ctx_f (comp_ctx_f c (Eprim_c v p l Hole_c)) b0) |[ e0
+                                                                        ]|) =
+                (rename_all_ctx_ns sig
+              (inlined_ctx_f c b0) |[ Eprim v p (apply_r_list sig l) e0 ]|)) by ctx_inl_push.
+        inv H6.
+        destructAll.        
+        unfold ce; unfold ce'.
+        rewrite H7.
+        rewrite H8 in *.
+        auto.
+        unfold term_sub_inl_size in *.
+        simpl in H.
+        simpl. omega.        
+      - (* halt *)
+        inv H6.
+        simpl in *.
+        unfold ce.
+        unfold ce'.
+        split; auto.
+        apply rt_refl.                
+    Admitted.
+
+
+  
+    Theorem contractcases_corresp:
+      forall cl2 cl1 sig c im x count sub,
+      let ce := (app_ctx_f (rename_all_ctx_ns sig (inlined_ctx_f c im)) (Ecase x (cl1 ++ (rename_all_case sig cl2)))) in
+      unique_bindings ce ->
+      closed ce ->
+      c_count ce count ->
+      cmap_view_ctx sub c ->
+      inl_inv im sub ce ->
+      sig_inv_dom sig ce ->
+      forall cl2' count' im' oes pfe pfsub bp,
+       contractcases oes (fun rm cm es H => contract rm cm (fst (fst es)) (snd (fst es)) (snd es)) sig count im sub cl2 pfe pfsub = existT _ (cl2', count', im') bp ->
+      let ce' := (app_ctx_f (rename_all_ctx_ns sig (inlined_ctx_f c im')) (Ecase x (cl1 ++ cl2'))) in
+      gsr_clos ce ce' /\ c_count ce' count' /\ inl_inv im' sub ce'.
+    Proof.
+      induction cl2; intros; simpl in H5.
+      - inv H5; unfold ce in *; unfold ce' in *; split; auto.
+        apply rt_refl.                        
+      -         
+        destruct a.
+        remember (contract sig count e sub im) as con_e.        
+        destruct con_e.
+        destruct x0.
+        destruct p.
+        simpl in ce.
+        assert (Hcl1: (rename_all_ns sig (Ecase x cl1)) = Ecase x cl1 ). {
+          rewrite <- (proj1 (rename_all_no_shadow _)).
+          apply Disjoint_dom_rename_all.
+          
+              (* by sig inv dead using H4 *)
+              split. intro. intro.
+              inv H6.
+              inv H7.
+              apply H4 in H6.
+              apply not_bound_dead_or_free in H6.
+              inv H6.
+              2:               apply H0 in H7; inv H7.
+              unfold ce in H7.
+              apply num_occur_app_ctx in H7. destructAll; pi0.
+              inv H7.
+              apply num_occur_app_case in H12.
+              destructAll.
+              pi0.              
+              assert (~(occurs_free (Ecase x cl1)) x0).
+              apply not_occurs_not_free.
+              eapply num_occur_n.
+              constructor; eauto.
+              simpl. destruct (cps_util.var_dec x0 x). exfalso; auto. auto.
+              auto.
+              (* using H4 *)
+              eapply sig_inv_dom_mon.
+              2: apply H4.
+              unfold ce.
+              rewrite bound_var_app_ctx.
+              rewrite bound_var_Ecase_app.
+              auto with Ensembles_DB.
+        }        
+        assert (rename_all_ctx_ns sig (inlined_ctx_f c im)
+               |[ Ecase x  (cl1 ++ (v, rename_all_ns sig e) :: rename_all_case sig cl2) ]| =
+                rename_all_ctx_ns sig (inlined_ctx_f (comp_ctx_f c (Ecase_c x cl1 v Hole_c cl2)) im)
+               |[ rename_all_ns sig e]|).
+        {
+          assert (
+              Ecase x (cl1 ++ (v, rename_all_ns sig e) :: rename_all_case sig cl2) =
+              rename_all_ns sig (Ecase x (cl1 ++ (v, e) :: cl2))).
+          {
+            simpl. rewrite list_append_map.
+            simpl in Hcl1. inversion Hcl1.
+            repeat rewrite H8. 
+            repeat rewrite H7.
+            reflexivity.
+          }
+          rewrite H6.
+          clear H6.
+          do 2 (rewrite <- (proj1 (rename_all_ns_app_ctx _ _))).
+          rewrite (proj1 inlined_comp_ctx).
+          simpl.          
+          rewrite <- app_ctx_f_fuse. 
+          simpl. reflexivity.
+        }
+        symmetry in Heqcon_e.
+        eapply shrink_corresp with
+        (c :=  (comp_ctx_f c (Ecase_c x cl1 v Hole_c cl2)))
+          in Heqcon_e; try (rewrite <- H6; auto).
+        Focus 2.
+        apply cmap_view_case. auto.
+
+        (* push Disjoint, Unique and Sub_inv through e0 *)
+        destructAll.
+        rewrite <- H6 in H7.
+        assert (Hub' := gsr_preserves_clos _ _ H H0 H7).
+        destructAll.
+        assert (Hse := gsr_preserves_sig_dom _ _ _ H H0 H7 H4).
+        assert (He0 : rename_all_ns sig e0 = e0). {
+              rewrite <- (proj1 (rename_all_no_shadow _)).
+              apply Disjoint_dom_rename_all.
+
+              split; intros; intro. inv H12.
+              inv H13. apply Hse in H12.
+              apply not_bound_dead_or_free in H12.
+              inv H12.
+              2: apply H11 in H13; inv H13.
+              
+              apply num_occur_app_ctx in H13; destructAll; pi0; auto.
+              apply not_occurs_not_free in H13. auto.
+              eapply sig_inv_dom_mon.
+              2: apply Hse.
+              rewrite bound_var_app_ctx.
+              right; auto.
+        }
+        
+        assert (
+            (rename_all_ctx_ns sig
+             (inlined_ctx_f (comp_ctx_f c (Ecase_c x cl1 v Hole_c cl2)) b0)
+            |[ rename_all_ns sig e0 ]|) =
+            (rename_all_ctx_ns sig
+                               (inlined_ctx_f c b0)
+            |[  (Ecase x ((cl1++[(v,e0)])++(rename_all_case sig cl2)))]|)).
+        {
+          assert (Ecase x ((cl1 ++ [(v, e0)]) ++ rename_all_case sig cl2)  =
+                  rename_all_ns sig (Ecase x ((cl1 ++ [(v, e0)]) ++ cl2))).
+          {
+            simpl.
+            inversion Hcl1.
+            rewrite list_append_map.
+            rewrite list_append_map.
+            simpl.
+            repeat rewrite H14.
+            repeat rewrite H13.
+            rewrite He0. reflexivity.
+          }
+          rewrite H12. clear H12.
+          
+          do 2 (rewrite <- (proj1 (rename_all_ns_app_ctx _ _))).
+          rewrite (proj1 inlined_comp_ctx).
+          simpl.          
+          rewrite <- app_ctx_f_fuse. 
+          simpl.
+          rewrite <- app_assoc. simpl. reflexivity.
+        }
+
+        (* I.H. *)
+
+        remember (contractcases oes
+             (fun (rm : r_map) (cm : c_map)
+                (es : prod (prod exp ctx_map) b_map)
+                (_ : lt (term_sub_inl_size es) (term_sub_inl_size oes)) =>
+              contract rm cm
+                (@fst exp ctx_map (@fst (prod exp ctx_map) b_map es))
+                (@snd exp ctx_map (@fst (prod exp ctx_map) b_map es))
+                (@snd (prod exp ctx_map) b_map es)) sig c0 b0 sub cl2
+             (@subcl_e_cons_l v e cl2
+                (@fst exp ctx_map (@fst (prod exp ctx_map) b_map oes))
+                (@eq_ind_r (list (prod var exp))
+                   (@cons (prod var exp) (@pair var exp v e) cl2)
+                   (fun x : list (prod var exp) =>
+                    subcl_e x
+                      (@fst exp ctx_map (@fst (prod exp ctx_map) b_map oes)))
+                   pfe (@cons (prod var exp) (@pair var exp v e) cl2)
+                   (@eq_refl (list (prod var exp))
+                      (@cons (prod var exp) (@pair var exp v e) cl2))))
+             (@sub_inl_size_compat sub im b0
+                (@snd exp ctx_map (@fst (prod exp ctx_map) b_map oes))
+                (@snd (prod exp ctx_map) b_map oes) pfsub b)) as cc_ind.
+        destruct cc_ind. destruct x0.
+        destruct p. 
+        symmetry in Heqcc_ind.
+        rewrite He0 in H12.
+        rewrite H12 in *.
+        
+        
+        eapply  IHcl2 in Heqcc_ind; eauto.
+        destruct Heqcc_ind.
+        destruct H14.
+        clear He0.
+        inv H5. unfold ce'.
+        split.
+        eapply rt_trans.
+        apply H7.
+        do 2 (rewrite <- app_assoc in H13).
+        simpl in H13.
+        rewrite <- app_assoc.
+        simpl.
+        auto.
+        rewrite <- app_assoc in H14.
+        rewrite <- app_assoc in H15.
+        split; auto.
+    Qed.
+
+
+
+
+
+       
+
+
+
+ 
+
+ Theorem inlined_fundefs_ctx_append1:
+   forall v f l fds_c im fds,
+ (inlined_fundefs_ctx_f
+             (fundefs_ctx_append (inlined_fundefs_f fds im)
+                (Fcons1_c v f l Hole_c (inlined_fundefs_f fds_c im))) im) = 
+(fundefs_ctx_append (inlined_fundefs_f fds im)
+                (Fcons1_c v f l Hole_c (inlined_fundefs_f fds_c im))).
+ Proof.
+   induction fds; intros; simpl; auto.
+   destruct (get_b v0 im); auto.
+   simpl. 
+   rewrite IHfds.
+   reflexivity.
+ Qed.
+
+
+ Theorem inlined_fundefs_ctx_append_shallow:
+   forall v f l fds_c b0 fds,     
+   (inlined_fundefs_ctx_f
+       (fundefs_ctx_append fds
+                           (Fcons1_c v f l Hole_c fds_c)) b0) =
+   (fundefs_ctx_append fds
+          (Fcons1_c v f l Hole_c fds_c)).
+ Proof.
+   intros.
+   induction fds.
+   - simpl.
+
+     rewrite IHfds. auto.
+   - simpl. reflexivity.
+ Qed.
+   
+   
+ 
+ Theorem rename_all_fundefs_ctx_append:
+   forall sig fdc fds,
+   rename_all_fun_ctx_ns sig (fundefs_ctx_append fds fdc) =
+   fundefs_ctx_append (rename_all_fun_ns sig fds)
+                      (rename_all_fun_ctx_ns sig fdc).
+ Proof.
+   induction fds; auto.
+   simpl.
+   rewrite IHfds. auto.
+ Qed.
+ 
+ Theorem app_f_ctx_fundefs_ctx_append:
+   forall fdc e fds,
+     fundefs_ctx_append fds fdc <[ e ]> =
+     fundefs_append fds (fdc <[e]>).
+ Proof.
+   induction fds; auto.
+   simpl; rewrite IHfds. auto.
+ Qed.
+
+ Print name_in_fundefs.
+
+ Fixpoint name_in_fundefs_ctx (B : fundefs_ctx) : Ensemble var :=
+  match B with
+    | Fcons1_c f' _ _ _ B0 => Union var [set f'] (name_in_fundefs B0)
+    | Fcons2_c f' _ _ _ B0 => Union var [set f'] (name_in_fundefs_ctx B0)
+  end.
+ 
+
+ 
+ Theorem bound_var_fundefs_ctx_append_f:
+   forall im fdc,
+   Included _ (name_in_fundefs_ctx fdc)
+            (bound_var_fundefs_ctx (inlined_fundefs_ctx_f fdc im)).
+ Proof.
+   induction fdc.
+   - simpl.
+     normalize_bound_var_ctx.
+     intro. intro. inv H; auto.
+     apply name_in_fundefs_bound_var_fundefs in H0.
+     auto.
+   - simpl.
+     normalize_bound_var_ctx.
+     intro; intro.
+     inv H; auto.
+ Qed.
+
+
+ Theorem name_in_fundefs_ctx_append:
+   forall fdc fds,
+   Same_set _ (name_in_fundefs_ctx (fundefs_ctx_append fds fdc)) (Union _ (name_in_fundefs fds) (name_in_fundefs_ctx fdc)).
+ Proof.
+   induction fds.
+   - simpl. rewrite IHfds; auto with Ensembles_DB.
+   - simpl. auto with Ensembles_DB.
+ Qed.
+
+ Theorem bound_var_fundefs_ctx_append:
+   forall fdc fds,
+   Same_set _ (bound_var_fundefs_ctx
+                 (fundefs_ctx_append fds fdc))
+        (Union _ (bound_var_fundefs fds) (bound_var_fundefs_ctx fdc)).
+ Proof.
+   induction fds; simpl; normalize_bound_var; try normalize_bound_var_ctx; eauto with Ensembles_DB.
+   rewrite IHfds.
+   eauto with Ensembles_DB.
+ Qed.   
+
+
+ Theorem name_in_fundefs_not_inlined:
+   forall f fds im,
+   name_in_fundefs fds f ->
+   get_b f im = false ->
+   bound_var_fundefs (inlined_fundefs_f fds im) f.
+ Proof.
+   induction fds; simpl; intros.
+   - inv H.
+     inv H1.
+     rewrite H0.
+     apply bound_var_fundefs_Fcons.
+     auto.
+     specialize (IHfds _ H1 H0).
+     destruct (get_b v im); eauto with Ensembles_DB.
+   - inv H.
+ Qed.     
+
+
+    Theorem postcontractfun_corresp:
+      forall fds_c fds e c im sub count sig,
+      let ce := (app_ctx_f (rename_all_ctx_ns sig (inlined_ctx_f (comp_ctx_f c (Efun1_c (fundefs_append fds fds_c) Hole_c)) im)) (rename_all_ns sig e)) in
+      unique_bindings ce ->
+      closed ce -> 
+      c_count ce count ->
+      cmap_view_ctx sub c ->
+      inl_inv im sub ce ->
+      sig_inv_dom sig ce ->
+      forall oes fds_c' count' im' pfe pfsub bp,
+       postcontractfun oes (fun rm cm es H => contract rm cm (fst (fst es)) (snd (fst es)) (snd es)) sig count im sub fds_c pfe pfsub = existT _ (fds_c', count', im')  bp ->
+       let ce' := (app_ctx_f (rename_all_ctx_ns sig (inlined_ctx_f (comp_ctx_f c (Efun1_c (fundefs_append fds fds_c') Hole_c)) im')) (rename_all_ns sig e)) in
+      gsr_clos ce ce' /\ c_count ce' count' /\ inl_inv im' sub ce'.
+    Proof.
+      induction fds_c; intros.
+      Focus 2.
+      simpl in H5. inv H5.
+      unfold ce in *; unfold ce'.
+      split; auto.
+      apply rt_refl.      
+      simpl in H5.
+      destruct (get_b v im) eqn:gbvim.
+      - (* get_b v im = true *)
+        assert (
+          (inlined_ctx_f
+             (comp_ctx_f c
+                (Efun1_c (fundefs_append fds (Fcons v f l e fds_c)) Hole_c))
+             im) =
+          (inlined_ctx_f
+             (comp_ctx_f c (Efun1_c (fundefs_append fds fds_c) Hole_c))
+             im)).
+        { do 2 (rewrite (proj1 inlined_comp_ctx)).
+          simpl.
+          do 2 (rewrite inlined_fundefs_append).
+          simpl.
+          rewrite gbvim.
+          reflexivity.
+        }
+        unfold ce in *.
+        rewrite H6 in *.        
+        eapply IHfds_c in H5; eauto.        
+      - (* get_b v im = false *)
+        destruct (get_c v count) eqn:gvc.
+        + (* get_c v count = 0 i.e. dead fun *)
+          assert (Hgsr_dead: gsr_clos ce (rename_all_ctx_ns sig
+                                                 (inlined_ctx_f
+                                                    (comp_ctx_f c
+                                                                (Efun1_c (fundefs_append fds fds_c) Hole_c))
+                                                    im) |[ rename_all_ns sig e0 ]|)).
+          {
+            (* by Fun_rem_s *)
+            unfold ce.
+            do 2 (rewrite (proj1 inlined_comp_ctx)).
+            simpl.
+            do 2 (rewrite inlined_fundefs_append).
+            simpl. rewrite gbvim.
+            do 2 (rewrite (proj1 (rename_all_ctx_ns_comp_ctx _ _))).
+            do 2 (rewrite <- app_ctx_f_fuse).
+            constructor. constructor.
+            simpl.
+            do 2 (rewrite rename_all_ns_fundefs_append).
+            simpl.
+            apply Fun_rem_s.
+            specialize (H1 v).
+            rewrite gvc in H1.
+            unfold ce in H1.
+            rewrite (proj1 inlined_comp_ctx) in H1.
+            simpl in H1.
+            rewrite (inlined_fundefs_append) in H1.
+            rewrite (proj1 (rename_all_ctx_ns_comp_ctx _ _)) in H1.
+            rewrite <- app_ctx_f_fuse in H1.
+            apply num_occur_app_ctx in H1.
+            destructAll; pi0.
+            simpl in H6.
+            rewrite rename_all_ns_fundefs_append in H6.
+            rewrite gbvim in H6.
+            simpl in H6.
+            auto.
+          }
+          assert (Ht := gsr_preserves_clos _ _ H H0 Hgsr_dead).
+          destruct Ht as (Hub_dead, Hdj_dead).  
+          assert (Hsig_dead := gsr_preserves_sig_dom _ _ _ H H0 Hgsr_dead H4).
+
+          (* I.H. *)
+          eapply IHfds_c in H5; eauto.
+          * destructAll.
+            unfold ce'; split; auto.
+            eapply rt_trans; eauto.
+          * intro.
+            specialize (H1 v0).
+            unfold ce in H1.
+            repeat normalize_ctx.
+            apply num_occur_app_ctx in H1.
+            destructAll.
+            apply num_occur_ec_comp_ctx in H1.
+            destructAll.
+            simpl in H8.
+            repeat normalize_ctx.
+            inv H8.
+            rewrite gbvim in H14.
+            apply fundefs_append_num_occur' in H14. destructAll.
+            simpl in H9. inv H9.
+            eapply num_occur_n.
+            apply num_occur_app_ctx. eexists; eexists.
+            split.
+            apply num_occur_ec_comp_ctx.
+            eexists; eexists.
+            split; eauto.
+            simpl.
+            repeat normalize_ctx.
+            split. constructor; eauto.
+            eapply fundefs_append_num_occur.  reflexivity.
+            eauto. eauto.
+            reflexivity.
+            split; eauto.
+            unfold dec_census.
+            
+            rewrite <- ((proj1 combine_minus_census_correct) _ _ _).
+            rewrite gccombine_sub. rewrite H7.
+            assert (get_c v0 (init_census (rename_all sig e)) = n0).
+            eapply (proj1 (num_occur_det _)).
+            apply init_census_correct.
+            rewrite (proj1 (rename_all_no_shadow _)).
+            auto.
+            intro. intros.
+            apply H4 in H9.
+            intro. apply H9.
+            unfold ce.
+            repeat (normalize_ctx; simpl).
+            rewrite gbvim.
+            apply bound_var_app_ctx.
+            left.
+            repeat normalize_bound_var_ctx.
+            right.
+            left.            
+            rewrite fundefs_append_bound_vars.
+            2: reflexivity.
+            right.
+            simpl.
+            normalize_bound_var.
+            rewrite <- (proj1 (bound_var_rename_all_ns _)).
+            auto.
+            rewrite H9. omega.
+          * intro. intro.
+            apply H3 in H6.
+            unfold ce in H6.
+            destruct H6.
+            split.
+            {
+              intro.
+              apply H6.
+              apply bound_var_app_ctx in H8.
+              apply bound_var_app_ctx.
+              inv H8.
+              left.
+              repeat (normalize_ctx; simpl).
+              rewrite gbvim.
+              simpl.
+              rewrite (proj1 (bound_var_ctx_comp_ctx)).
+              rewrite (proj1 (bound_var_ctx_comp_ctx)) in H9.
+              inv H9; auto.
+              right.
+              normalize_bound_var_ctx'.
+              simpl in H8.
+              repeat (normalize_ctx; simpl).
+              rewrite fundefs_append_bound_vars.
+              2: reflexivity.
+              normalize_bound_var.
+              normalize_bound_var_ctx_in_ctx'.
+              rewrite fundefs_append_bound_vars in H8.
+              2: reflexivity.
+              destruct H8.
+              left. 
+              destruct H8; auto.
+              auto.
+              right. auto.              
+            }
+            {
+              intros.
+              apply H7 in H8.
+              eapply Disjoint_Included_l.
+              2: apply H8.
+              repeat (normalize_ctx; simpl).
+              do 2 (rewrite bound_var_app_ctx).
+              do 2 (rewrite (proj1 bound_var_ctx_comp_ctx)).
+              repeat normalize_bound_var_ctx'.
+              rewrite fundefs_append_bound_vars.
+              2: reflexivity.
+              intro. intros.
+              rewrite fundefs_append_bound_vars.
+              2: reflexivity.
+              rewrite gbvim.
+              simpl.
+              repeat normalize_bound_var.
+              destruct H9; auto.
+              destruct H9; auto.
+              destruct H9; auto.
+              destruct H9; auto.
+              eauto 25 with Ensembles_DB.
+            }
+        + (* get_c v count = (S n) *)
+          (* contract on e *)
+          remember  (contract sig count e sub im).
+          destruct s.
+          destruct x.
+          destruct p.
+          symmetry in Heqs.
+          assert (
+              rename_all_ctx_ns sig
+                                (inlined_ctx_f
+                                   (comp_ctx_f c
+                                               (Efun1_c (fundefs_append fds (Fcons v f l e fds_c)) Hole_c))
+                                   im) |[ rename_all_ns sig e0 ]| =
+             (rename_all_ctx_ns sig (inlined_ctx_f (comp_ctx_f c ( 
+                                              Efun2_c  (fundefs_ctx_append (inlined_fundefs_f fds im) (Fcons1_c v f l Hole_c (inlined_fundefs_f fds_c im))) e0)) im) |[ rename_all_ns sig e ]|)).
+          { 
+            do 2 (rewrite <- (proj1 (rename_all_ns_app_ctx _ _))).
+            repeat normalize_ctx.
+            simpl.
+            do 2 (rewrite <- app_ctx_f_fuse).
+            simpl.
+            repeat normalize_ctx.
+            simpl.
+            rewrite gbvim.
+            simpl.
+            rewrite inlined_fundefs_ctx_append1.
+            rewrite rename_all_fundefs_ctx_append.
+            rewrite app_f_ctx_fundefs_ctx_append.
+            simpl.
+            reflexivity.
+          }
+          unfold ce in *; rewrite H6 in *.
+          
+
+          eapply shrink_corresp in Heqs; eauto.
+          (* can add shallow Efun2_c *)
+          2: (apply cmap_view_efun2; auto).
+          
+          
+          (* I H *)
+          destruct Heqs.
+          destruct H8.
+          assert (Ht := gsr_preserves_clos _ _ H H0 H7).
+          destruct Ht as (Hub_post, Hdj_post).
+          assert (Hsig_post := gsr_preserves_sig_dom _ _ _ H H0 H7 H4).
+          
+          
+
+          assert (He1 : e1 = rename_all_ns sig e1).
+          {
+            rewrite <- (proj1 (rename_all_no_shadow _)).
+            symmetry.
+            apply rename_sig_dead.
+            intro.             intros.
+            apply Hsig_post in H10.
+            destructAll.
+            apply not_bound_dead_or_free in H10.
+            inv H10.
+            2: apply Hdj_post in H11; inv H11.
+            
+            apply num_occur_app_ctx in H11.
+            destructAll; pi0.
+            auto.
+            eapply sig_inv_dom_mon.
+            2: apply Hsig_post.
+            rewrite bound_var_app_ctx.
+            right;
+            auto.
+          }
+          
+          
+          assert
+            ( (rename_all_ctx_ns sig
+              (inlined_ctx_f
+                 (comp_ctx_f c
+                    (Efun2_c
+                       (fundefs_ctx_append (inlined_fundefs_f fds im)
+                          (Fcons1_c v f l Hole_c (inlined_fundefs_f fds_c im)))
+                       e0)) b0) |[ e1 ]|) =
+           (rename_all_ctx_ns sig
+              (inlined_ctx_f
+                 (comp_ctx_f c
+                    (Efun1_c
+                       (fundefs_append (fundefs_append fds (Fcons v f l e1 Fnil)) fds_c) Hole_c)) b0) |[ rename_all_ns sig e0 ]|)).
+          { 
+            rewrite He1 at 1.
+            clear He1.
+            repeat (normalize_ctx; simpl).
+            destruct (get_b v b0) eqn:gvb0.
+            - apply H9 in gvb0.
+              destructAll.
+              exfalso.
+              apply H10.
+              apply bound_var_app_ctx.
+              left.
+              normalize_bound_var_ctx.
+              right.
+              simpl.
+              normalize_bound_var_ctx.
+              left.
+              rewrite <- (proj2 (bound_var_ctx_rename_all_ns _)).
+              apply bound_var_fundefs_ctx_append_f.
+              apply name_in_fundefs_ctx_append.
+              right. simpl. auto.
+            - simpl.
+              do 2 (rewrite <- app_ctx_f_fuse).
+              simpl.
+              assert ((inlined_fundefs_ctx_f
+                         (fundefs_ctx_append (inlined_fundefs_f fds im)
+                                             (Fcons1_c v f l Hole_c (inlined_fundefs_f fds_c im))) b0)  =
+                      fundefs_ctx_append (inlined_fundefs_f fds b0)
+                                         (Fcons1_c v f l Hole_c (inlined_fundefs_f fds_c b0))).
+              {
+                rewrite inlined_fundefs_ctx_append_shallow.
+                erewrite eq_b_inlined_fundefs.
+                erewrite eq_b_inlined_fundefs with (fds := fds_c).
+                reflexivity.
+                {
+                  intro.
+                  intro.
+                  destruct (get_b x b0) eqn:gxb0.
+                  destruct (get_b x im) eqn:gxim.
+                  reflexivity.
+                
+                  (* prove that this is false *)
+                  exfalso.
+                  apply H9 in gxb0.
+                  destruct gxb0.
+                  apply H11.
+                  apply bound_var_app_ctx.
+                  left.
+                  SearchAbout bound_var_ctx comp_ctx_f.
+                  apply bound_var_ctx_comp_ctx.
+                  right.
+                  simpl.
+                  rewrite inlined_fundefs_ctx_append_shallow.
+                  normalize_bound_var_ctx.
+                  left.
+                  rewrite <- (proj2 (bound_var_ctx_rename_all_ns  _)).
+                  rewrite bound_var_fundefs_ctx_append.
+                  right.
+                  apply bound_var_Fcons1_c.
+                  right. right.
+                  right.
+                  apply name_in_fundefs_not_inlined; auto.
+
+                  destruct (get_b x im) eqn:gxim.
+                  assert (H' := b).
+                  apply b_map_le_c in H'.
+                  simpl in H'.
+                  apply H' in gxim.
+                  rewrite gxim in gxb0.  auto.
+                  reflexivity.
+                } 
+                {
+                  intro.
+                  intro.
+                  destruct (get_b x b0) eqn:gxb0.
+                  destruct (get_b x im) eqn:gxim.
+                  reflexivity.
+                
+                  (* prove that this is false *)
+                  exfalso.
+                  apply H9 in gxb0.
+                  destruct gxb0.
+                  apply H11.
+                  apply bound_var_app_ctx.
+                  left.
+                  apply bound_var_ctx_comp_ctx.
+                  right.
+                  simpl.
+                  rewrite inlined_fundefs_ctx_append_shallow.
+                  normalize_bound_var_ctx.
+                  left.
+                  rewrite <- (proj2 (bound_var_ctx_rename_all_ns  _)).
+                  rewrite bound_var_fundefs_ctx_append.
+                  left.
+                  apply name_in_fundefs_not_inlined; auto.
+
+                  destruct (get_b x im) eqn:gxim.
+                  assert (H' := b).
+                  apply b_map_le_c in H'.
+                  simpl in H'.
+                  apply H' in gxim.
+                  rewrite gxim in gxb0.  auto.
+                  reflexivity.
+                } 
+              }
+              rewrite H10.
+              rewrite rename_all_fundefs_ctx_append.
+              simpl.
+              rewrite app_f_ctx_fundefs_ctx_append. simpl.
+              rewrite <- fundefs_append_assoc.
+              simpl. reflexivity.
+          }
+
+          rewrite H10 in *.
+          remember ( postcontractfun oes
+             (fun (rm : r_map) (cm : c_map)
+                (es : prod (prod exp ctx_map) b_map)
+                (_ : lt (term_sub_inl_size es) (term_sub_inl_size oes)) =>
+              contract rm cm
+                (@fst exp ctx_map (@fst (prod exp ctx_map) b_map es))
+                (@snd exp ctx_map (@fst (prod exp ctx_map) b_map es))
+                (@snd (prod exp ctx_map) b_map es)) sig c0 b0 sub fds_c
+             (@subfds_Fcons v f l e fds_c
+                (@fst exp ctx_map (@fst (prod exp ctx_map) b_map oes))
+                (@eq_ind_r fundefs (Fcons v f l e fds_c)
+                   (fun x : fundefs =>
+                    subfds_e x
+                      (@fst exp ctx_map (@fst (prod exp ctx_map) b_map oes)))
+                   pfe (Fcons v f l e fds_c)
+                   (@eq_refl fundefs (Fcons v f l e fds_c))))
+             (@tsis_sub_pcf' sub im
+                (@snd exp ctx_map (@fst (prod exp ctx_map) b_map oes))
+                (@snd (prod exp ctx_map) b_map oes) b0 pfsub b)).
+          destruct s.
+          destruct x.
+          destruct p.
+          symmetry in Heqs.
+          eapply IHfds_c  in Heqs; eauto.
+          clear He1.
+          destructAll.
+          inv H5.
+          unfold ce'.
+          split; auto.
+          eapply rt_trans.
+          apply H7.
+          rewrite <- fundefs_append_assoc in H11.
+          rewrite <- fundefs_append_assoc in H11. simpl in H11.
+          rewrite <- fundefs_append_assoc.  simpl.
+           auto.
+          split; auto.
+          rewrite <- fundefs_append_assoc in H12.
+          auto.
+          rewrite <- fundefs_append_assoc in H13.
+          auto.
+    Qed.
+
+    (* 
+    Theorem shrink_corresp_top:
+      forall e,
+      unique_bindings e ->
+      closed e ->
+      gsr_clos e (shrink_top e).
+    Proof.
+      intros.
+      unfold shrink_top.
+      eapply shrink_corresp with (c := Hole_c); auto.
+      rewrite <- (proj1 rename_all_empty).
+      rewrite Disjoint_inlined_ctx.
+      simpl. reflexivity.
+      rewrite bound_var_Hole_c.
+      apply Disjoint_Empty_set_l.
+      apply init_census_correct.
+      apply empty_view_hole.
+      {
+        intro.
+        intro.
+        unfold get_b in H1.
+        rewrite M.gempty in H1. inv H1.
+      }
+      {
+        intro. intros.
+        rewrite M.gempty in H1.
+        inv H1.
+      }
+    Qed.
+
+*)
+
+    End CONTRACT.
